mtms: fix adequacy

theories/examples/mem_trans_msg_send/adequacy.v
@@ -4,61 +4,58 @@ From HypVeri Require Import machine_extra lifting.
 From HypVeri.algebra Require Import base mailbox pagetable mem.
 From HypVeri.lang Require Import reg_extra.
 From HypVeri.examples Require Import instr utils.
-From HypVeri.logrel Require Import logrel logrel_extra.
+From HypVeri.logrel Require Import logrel logrel_extra logrel_prim_extra.
 From HypVeri.examples.mem_trans_msg_send Require Import proof.
-From HypVeri.examples.mem_trans_msg_send Require Import ftlr.
 Require Import Setoid.
 
 Section mtms_adequacy.
   Context `{hypparams: !HypervisorParameters}.
+  Context (p_prog0 p_prog1 p_prog2 : PID).
+  Context (p_tx0 p_rx0 p_tx1 p_rx1 p_tx2 p_rx2 : PID).
+  Context (p_share : PID).
+  Context (Hps_nd: NoDup [p_prog0;p_prog1;p_prog2;p_share;p_tx0;p_tx1;p_tx2;p_rx0;p_rx1;p_rx2]).
+  Context (addr : Imm) (Heq_pshare : of_pid p_share = addr).
+  Context (i_ptx0 : Imm) (Heq_ptx0 : of_pid p_tx0 = i_ptx0).
+  Context (i_prx1 : Imm) (Heq_prx1 : of_pid p_rx1 = i_prx1).
+  Context (σ : state).
   
-  Definition pgt (σ : state) (p_prog1 p_prog2 p_prog3 p_tx1 p_tx2 p_tx3 p_rx1 p_rx2 p_rx3 p : PID) :=    
-    access_layout σ {[V0 := to_dfrac_agree (DfracOwn 1) {[p; p_prog1; p_tx1]};
-                     V1 := to_dfrac_agree (DfracOwn 1) {[p_prog2; p_tx2; p_rx2]};
-                     V2 := to_dfrac_agree (DfracOwn 1) {[p_tx3; p_rx3; p_prog3]}]} ∧
-    excl_layout σ {[p_rx1 := true; p_rx2 := true; p_rx3 := true; p_tx3 := true; p_prog3 := true; p:= true]} ∧
-    own_layout σ {[p_rx1 := None; p_rx2 := None; p_rx3 := None; p_tx3 := None; p_prog3 := Some V2; p:= Some V0]}.  
+  Definition pgt :=
+    access_layout σ {[V0 := to_dfrac_agree (DfracOwn 1) {[p_share; p_prog0; p_tx0]};
+                     V1 := to_dfrac_agree (DfracOwn 1) {[p_prog1; p_tx1; p_rx1]};
+                     V2 := to_dfrac_agree (DfracOwn 1) {[p_tx2; p_rx2; p_prog2]}]} ∧
+    excl_layout σ {[p_rx0 := true; p_rx1 := true; p_rx2 := true; p_tx2 := true; p_prog2 := true; p_share:= true]} ∧
+    own_layout σ {[p_rx0 := None; p_rx1 := None; p_rx2 := None; p_tx2 := None; p_prog2 := Some V2; p_share:= Some V0]}.
 
-  Program Definition mem (σ : state) (p_prog1 p_prog2 p_prog3 p_tx1 p_tx2 p_tx3 p_rx1 p_rx2 p_rx3 : PID) (addr txbase rxbase : Imm) :=
+  Program Definition mem:=
     let mem := ((get_mem σ): gmap Addr Word)  in
-    (∀ (m : gmap Addr Addr), dom m = set_of_addr {[p_prog1]} -> m ⊆ mem -> m = mem_page_program p_prog1 (lending_program0 addr txbase) _) ∧
-    (∀ (m : gmap Addr Addr), dom m = set_of_addr {[p_prog2]} -> m ⊆ mem -> m = mem_page_program p_prog2 (lending_program1 addr rxbase) _) ∧
-    ((set_of_addr {[p_prog1;p_prog2; tpa addr; p_prog3;p_tx1; p_tx2; p_tx3;p_rx1;p_rx2;p_rx3]}) ⊆ dom mem).
+    (∀ (m : gmap Addr Addr), dom m = set_of_addr {[p_prog0]} -> m ⊆ mem -> m = mem_page_program p_prog0 (mtms_program0 addr i_ptx0) _) ∧
+    (∀ (m : gmap Addr Addr), dom m = set_of_addr {[p_prog1]} -> m ⊆ mem -> m = mem_page_program p_prog1 (mtms_program1 addr i_prx1) _) ∧
+    ((set_of_addr {[p_prog0;p_prog1; p_share; p_prog2;p_tx0; p_tx1; p_tx2;p_rx0;p_rx1;p_rx2]}) ⊆ dom mem).
   Next Obligation. lia. Qed.
   Next Obligation. lia. Qed.  
   
-  Definition regs (σ : state) (p_prog1 p_prog2 : PID)
-    := reg_layout σ ({[PC:=of_pid p_prog1]}) V0
-       ∧ reg_layout σ ({[PC:=of_pid p_prog2]}) V1
+  Definition regs
+    := reg_layout σ ({[PC:=of_pid p_prog0]}) V0
+       ∧ reg_layout σ ({[PC:=of_pid p_prog1]}) V1
        ∧ ∀ i rn, is_Some (((get_reg_files σ) !!! i) !! rn).
   
-  Definition mailbox (σ: state) (p_tx1 p_tx2 p_tx3 p_rx1 p_rx2 p_rx3 : PID):=
-    mailbox_layout σ {[(V0, TX) := p_tx1; (V1, TX) := p_tx2; (V2, TX) := p_tx3;
-                      (V0, RX) := p_rx1; (V1, RX) := p_rx2; (V2, RX) := p_rx3]} ∧
+  Definition mailbox:=
+    mailbox_layout σ {[(V0, TX) := p_tx0; (V1, TX) := p_tx1; (V2, TX) := p_tx2;
+                      (V0, RX) := p_rx0; (V1, RX) := p_rx1; (V2, RX) := p_rx2]} ∧
     rx_layout σ {[V0 := None; V1 := None; V2 := None]}.
   
-  Definition transactions (σ: state):=
-    dom (get_transactions σ) = valid_handles ∧
-    map_Forall (λ k v, v = None) (get_transactions σ).  
+  Definition transactions := σ.2 = {[W0 := None]}.
 
-  Definition initial_config (σ: state) (ms: list exec_mode) (φs : list (exec_mode -> Prop )):=
+  Definition initial_config (ms: list exec_mode) (φs : list (exec_mode -> Prop)):=
                   (get_current_vm σ) = V0 ∧
                   φs = [(λ m , m = HaltI); (λ _, False); (λ _, True)] ∧
                   ms = [ExecI;ExecI;ExecI] ∧
-                    (∃ (p_prog1 p_prog2 p_prog3 p_tx1 p_tx2 p_tx3 p_rx1 p_rx2 p_rx3 : PID) (addr txbase rxbase : Imm),
-                    of_pid p_tx1 = of_imm txbase ∧ of_pid p_rx2 = of_imm rxbase ∧ of_pid (tpa addr) = (of_imm addr) ∧    
-                    NoDup' [p_prog1;p_prog2;p_prog3;p_tx1;p_tx2;p_tx3;p_rx1;p_rx2;p_rx3; tpa addr] ∧
-                    (pgt σ p_prog1 p_prog2 p_prog3 p_tx1 p_tx2 p_tx3 p_rx1 p_rx2 p_rx3 (tpa addr)) ∧
-                    (mem σ p_prog1 p_prog2 p_prog3 p_tx1 p_tx2 p_tx3 p_rx1 p_rx2 p_rx3 addr txbase rxbase) ∧
-                    (regs σ p_prog1 p_prog2) ∧
-                    (mailbox σ p_tx1 p_tx2 p_tx3 p_rx1 p_rx2 p_rx3)
-                  ) ∧
-                  transactions σ.
+                    pgt ∧ mem ∧ regs ∧ mailbox ∧ transactions.
   
-  Context {vm_preG: gen_VMPreG Addr VMID Word reg_name PID transaction_type irisΣ}.      
+  Context {vm_preG: gen_VMPreG Addr VMID Word reg_name PID transaction_type irisΣ}.
 
   Lemma memory_list_gmap (pid : PID) (mem_list : list Word) (Hle: length mem_list < (Z.to_nat page_size))
-        (mem_gmap : gmap Addr Word) (σ : state)
+        (mem_gmap : gmap Addr Word)
         (H : NoDup (zip (finz.seq pid (length mem_list)) mem_list).*1)
         (G : mem_gmap = mem_page_program pid mem_list Hle)
         γ :
@@ -76,7 +73,7 @@ Section mtms_adequacy.
       lia.
   Qed.  
 
-  Lemma get_reg_gmap_split σ γ:
+  Lemma get_reg_gmap_split γ:
     ([∗ map] p↦w ∈ (get_reg_gmap σ) , p ↪[γ] w)%I ⊢ [∗ list] i ∈ ((list_of_vmids): list VMID), [∗ map] p↦w ∈ get_reg_gmap_vm σ i, p ↪[γ] w.
   Proof.
     iIntros "Hmap".
@@ -134,25 +131,22 @@ Section mtms_adequacy.
   Qed.  
   
   (* exec_mode of all VMs *)
-  Lemma adequacy (σ : state) (ms : list exec_mode) φs:
+  Lemma adequacy (ms : list exec_mode) φs:
     (* we need assumptions to be able to allocate resources *)
     (* with these resources, we apply the specification and get the wptp *)
     (* along with some other stuff, then it should be enough to apply the adequacy theorem *)
-    (initial_config σ ms φs) ->
+    (initial_config ms φs) ->
     adequate ms σ ((λ φ, λ v _, φ v)<$> φs).
     (* φ : vm 0 is scheduled but halted *)
   Proof.
     intros Hinit.
+    destruct Hinit as (Hcur & -> & -> & Hpgt & Hmem & Hreg & Hmb & Htrans).
     set (saved_props := (let (_, x, _, _) := iris_subG irisΣ (subG_refl irisΣ) in x)).
     set (prop_name := (let (_, _, x, _) := iris_subG irisΣ (subG_refl irisΣ) in x)).
-
     set (name_map := (let (_, _, _, x) := iris_subG irisΣ (subG_refl irisΣ) in x)).
     eapply (wp_adequacy irisΣ); auto.
-    destruct Hinit as (Hcur & -> & -> & (p1 & p2 & p1p2ne & Hpgt & Hmem & Hreg) & Htrans).
-    by simpl.
     intro Hinv.
     iIntros.
-    destruct Hinit as ( Hcur & Hinit).
     iMod (gen_mem_alloc σ) as (mem_gname) "[Hσmem Hmem]".
     iMod (gen_reg_alloc σ) as (reg_gname) "[Hσreg Hreg]".
     iMod (gen_mb_alloc σ) as (mb_gname) "[Hσmb Hmb]".
@@ -170,7 +164,6 @@ Section mtms_adequacy.
                   own_gname access_gname excl_gname trans_gname hpool_gname retri_gname)) as VMG.
     iExists (gen_vm_interp (Σ := irisΣ)).
     
-    destruct Hinit as (-> & -> & (p_prog1 & p_prog2 & p_prog3 & p_tx1 & p_tx2 & p_tx3 & p_rx1 & p_rx2 & p_rx3 & addr & txbase & rxbase & Heqtx & Heqrx & Heqaddr & Hnodup_p & Hpgt & Hmem & Hreg & (Hmb & Hrx)) & Htrans).
     destruct Hreg as (Hlookup_reg0 & Hlookup_reg1 & Htotal_reg).
     
     (* use assumptions to extract resources *)
@@ -198,7 +191,7 @@ Section mtms_adequacy.
     pose proof (Htotal_reg V0 R4) as [r4_ Hlookup_reg0_r4].
     pose proof (Htotal_reg V0 R5) as [r5_ Hlookup_reg0_r5].
       
-    iDestruct (big_sepM_subseteq _ (get_reg_gmap_vm σ V0) {[(PC, V0):= (of_pid p_prog1); (R0, V0) := r0_;
+    iDestruct (big_sepM_subseteq _ (get_reg_gmap_vm σ V0) {[(PC, V0):= (of_pid p_prog0); (R0, V0) := r0_;
                                  (R1,V0):= r1_; (R2,V0):= r2_; (R3,V0):= r3_; (R4,V0):= r4_; (R5,V0):= r5_]} with "Hreg0") as "Hreg0";eauto.
     {
       apply (λ x, reg_layout_extend σ _ _ x R5 r5_ Hlookup_reg0_r5) in Hlookup_reg0.
@@ -248,7 +241,7 @@ Section mtms_adequacy.
     pose proof (Htotal_reg V1 R3) as [r3__ Hlookup_reg1_r3].
     pose proof (Htotal_reg V1 R4) as [r4__ Hlookup_reg1_r4].
     pose proof (Htotal_reg V1 R5) as [r5__ Hlookup_reg1_r5].
-    iDestruct (big_sepM_subseteq _ (get_reg_gmap_vm σ V1) {[(PC, V1):= (of_pid p_prog2); (R0, V1) := r0__; (R1, V1) := r1__; (R2, V1) := r2__; (R3, V1) := r3__; (R4, V1) := r4__; (R5, V1) := r5__]} with "Hreg1") as "Hreg1";eauto.
+    iDestruct (big_sepM_subseteq _ (get_reg_gmap_vm σ V1) {[(PC, V1):= (of_pid p_prog1); (R0, V1) := r0__; (R1, V1) := r1__; (R2, V1) := r2__; (R3, V1) := r3__; (R4, V1) := r4__; (R5, V1) := r5__]} with "Hreg1") as "Hreg1";eauto.
     {
       apply (λ x, reg_layout_extend σ _ _ x R5 r5__ Hlookup_reg1_r5) in Hlookup_reg1.
       apply (λ x, reg_layout_extend σ _ _ x R4 r4__ Hlookup_reg1_r4) in Hlookup_reg1.
@@ -287,10 +280,10 @@ Section mtms_adequacy.
     iDestruct (big_sepM_insert with "Hreg1") as "(R51 & _)".
     { rewrite lookup_empty; eauto. }
 
-    iDestruct (big_sepM_subseteq _ (get_mb_gmap σ) {[(V0, TX):= p_tx1; (V1, TX) := (p_tx2); (V2, TX) := (p_tx3); (V0, RX) := p_rx1; (V1, RX) := p_rx2; (V2, RX) := p_rx3]} with "Hmb") as "Hmb";eauto.
+    iDestruct (big_sepM_subseteq _ (get_mb_gmap σ) {[(V0, TX):= p_tx0; (V1, TX) := (p_tx1); (V2, TX) := (p_tx2); (V0, RX) := p_rx0; (V1, RX) := p_rx1; (V2, RX) := p_rx2]} with "Hmb") as "Hmb";eauto.
     {
       apply mailbox_layout_get_mb_gmap.
-      assumption.
+      apply Hmb.
     }
     iDestruct (big_sepM_insert with "Hmb") as "(mb0TX & Hmb)".
     { rewrite !lookup_insert_None; split; eauto. }
@@ -308,7 +301,7 @@ Section mtms_adequacy.
     iDestruct (big_sepM_subseteq _ (get_rx_gmap σ) {[V0:= None; V1 := None; V2 := None]} with "Hrxs") as "Hrxs";eauto.
     {
       apply rx_layout_get_rx_gmap.
-      assumption.
+      apply Hmb.
     } 
     iDestruct (big_sepM_insert with "Hrxs") as "(RX0St & Hrxs)".
     { rewrite !lookup_insert_None; split; eauto. }
@@ -329,8 +322,23 @@ Section mtms_adequacy.
       apply map_union_subseteq_r.
       done.
     }    
-    
-    pose proof (union_split_difference_intersection_subseteq_L {[p_prog1; p_prog2; tpa addr; p_prog3; p_tx1; p_tx2; p_tx3; p_rx1; p_rx2; p_rx3]} {[p_prog1]}) as [Heq Hdisj].
+
+    assert (NoDup' [p_prog0;p_prog1;p_prog2;p_share;p_tx0;p_tx1;p_tx2;p_rx0;p_rx1;p_rx2]) as Hps_nd'.
+    {
+      rewrite /NoDup'.
+      intros. intro.
+      apply H1.
+      pose proof Hps_nd as Hps_nd'.
+      rewrite NoDup_alt in Hps_nd'.
+      apply lookup_lt_is_Some_2 in H.
+      apply lookup_lt_is_Some_2 in H0.
+      destruct H, H0.
+      rewrite H2 in H. rewrite H in H0. inversion H0;subst x0;clear H0.
+      eapply Hps_nd';eauto.
+      rewrite H2;done.
+    }
+
+    pose proof (union_split_difference_intersection_subseteq_L {[p_prog0; p_prog1; p_share; p_prog2; p_tx0; p_tx1; p_tx2; p_rx0; p_rx1; p_rx2]} {[p_prog0]}) as [Heq Hdisj].
     set_solver +.
     rewrite Heq in Hdom_mem2.
     rewrite set_of_addr_union in Hdom_mem2.    
@@ -338,10 +346,10 @@ Section mtms_adequacy.
     clear Heq.
     apply dom_union_inv_L in Hdom_mem2.
     2 : { apply set_of_addr_disj. done. }
-    destruct Hdom_mem2 as (mem1 & mem_p_prog1 & -> & Hmem1_disj  & Hdom_mem1 & Hdom_mem_p_prog1).
-    iDestruct ((big_sepM_union _ _) with "Hmem") as "(Hmem1 & mem_p_prog1)";auto.
+    destruct Hdom_mem2 as (mem1 & mem_p_prog0 & -> & Hmem1_disj  & Hdom_mem1 & Hdom_mem_p_prog0).
+    iDestruct ((big_sepM_union _ _) with "Hmem") as "(Hmem1 & mem_p_prog0)";auto.
     clear Hdisj.
-    pose proof (union_split_difference_intersection_subseteq_L ({[p_prog1; p_prog2; tpa addr; p_prog3; p_tx1; p_tx2; p_tx3; p_rx1; p_rx2; p_rx3]} ∖ {[p_prog1]}) {[p_prog2]}) as [Heq Hdisj].
+    pose proof (union_split_difference_intersection_subseteq_L ({[p_prog0; p_prog1; p_share; p_prog2; p_tx0; p_tx1; p_tx2; p_rx0; p_rx1; p_rx2]} ∖ {[p_prog0]}) {[p_prog1]}) as [Heq Hdisj].
     apply singleton_subseteq_l.
     rewrite !difference_union_distr_l_L.
     rewrite difference_diag_L.
@@ -357,11 +365,11 @@ Section mtms_adequacy.
     clear Heq.
     apply dom_union_inv_L in Hdom_mem1.
     2 : { apply set_of_addr_disj. done. }
-    destruct Hdom_mem1 as (mem2 & mem_p_prog2 &  -> & Hmem2_disj  & Hdom_mem2 & Hdom_mem_p_prog2).
+    destruct Hdom_mem1 as (mem2 & mem_p_prog1 &  -> & Hmem2_disj  & Hdom_mem2 & Hdom_mem_p_prog1).
     clear Hdisj.
-    iDestruct ((big_sepM_union _ _) with "Hmem1") as "(Hmem2 & mem_p_prog2)";auto.
+    iDestruct ((big_sepM_union _ _) with "Hmem1") as "(Hmem2 & mem_p_prog1)";auto.
 
-    pose proof (union_split_difference_intersection_subseteq_L (({[p_prog1; p_prog2; tpa addr; p_prog3; p_tx1; p_tx2; p_tx3; p_rx1; p_rx2; p_rx3]} ∖ {[p_prog1]}) ∖ {[p_prog2]}) {[tpa addr]}) as [Heq Hdisj].
+    pose proof (union_split_difference_intersection_subseteq_L (({[p_prog0; p_prog1; p_share; p_prog2; p_tx0; p_tx1; p_tx2; p_rx0; p_rx1; p_rx2]} ∖ {[p_prog0]}) ∖ {[p_prog1]}) {[p_share]}) as [Heq Hdisj].
     apply singleton_subseteq_l.
     rewrite !difference_union_distr_l_L.
     rewrite !difference_diag_L.
@@ -385,15 +393,15 @@ Section mtms_adequacy.
       | [ H : context G [?a ∖ ?b ∖ ?c ∖ ?d] |- _ ] => set p := a; set q := b; set r := c; set t := d
     end.
 
-    change {[p_prog1; p_prog2; p_prog3; p_tx1; p_tx2; p_tx3; p_rx1; p_rx2; p_rx3]} with p in Hdom_mem'.
-    change {[p_prog1]} with q in Hdom_mem'.
-    change {[p_prog2]} with r in Hdom_mem'.
-    change {[tpa addr]} with t in Hdom_mem'.
-    assert (p ∖ q ∖ r ∖ t = {[p_prog3; p_tx1; p_tx2; p_tx3; p_rx1; p_rx2; p_rx3]}) as Heq.
+    change {[p_prog0; p_prog1; p_prog2; p_tx0; p_tx1; p_tx2; p_rx0; p_rx1; p_rx2]} with p in Hdom_mem'.
+    change {[p_prog0]} with q in Hdom_mem'.
+    change {[p_prog1]} with r in Hdom_mem'.
+    change {[p_share]} with t in Hdom_mem'.
+    assert (p ∖ q ∖ r ∖ t = {[p_prog2; p_tx0; p_tx1; p_tx2; p_rx0; p_rx1; p_rx2]}) as Heq.
     {
-      assert (p ∖ q ∖ r = {[tpa addr; p_prog3; p_tx1; p_tx2; p_tx3; p_rx1; p_rx2; p_rx3]}) as ->.
+      assert (p ∖ q ∖ r = {[p_share; p_prog2; p_tx0; p_tx1; p_tx2; p_rx0; p_rx1; p_rx2]}) as ->.
       {
-        assert (p ∖ q = {[p_prog2; tpa addr; p_prog3; p_tx1; p_tx2; p_tx3; p_rx1; p_rx2; p_rx3]}) as ->.
+        assert (p ∖ q = {[p_prog1; p_share; p_prog2; p_tx0; p_tx1; p_tx2; p_rx0; p_rx1; p_rx2]}) as ->.
         {
           subst p q.
           rewrite !difference_union_distr_l_L.
@@ -420,76 +428,76 @@ Section mtms_adequacy.
       rewrite <-!difference_union_distr_l_L.
       rewrite difference_disjoint_L.
       - reflexivity.
-      - solve_NoDup 9.
+      - solve_NoDup 3.
     }    
     rewrite Heq in Hdom_mem'.
     clear Heq.
     rewrite set_of_addr_union in Hdom_mem'.
     2 : {
-      solve_NoDup 8.
+      solve_NoDup 9.
     }
     apply dom_union_inv_L in Hdom_mem'.
     2 : {
       apply set_of_addr_disj.
+      solve_NoDup 9.
+    }
+    destruct Hdom_mem' as (mem3 & mem_p_rx2 &  -> & Hmem3_disj  & Hdom_mem1 & Hdom_mem_p_rx2).
+    iDestruct ((big_sepM_union _ _) with "Hmem") as "(Hmem2 & p_rx2)";auto.
+    rewrite set_of_addr_union in Hdom_mem1.
+    2 : {
       solve_NoDup 8.
     }
-    destruct Hdom_mem' as (mem3 & mem_p_rx3 &  -> & Hmem3_disj  & Hdom_mem1 & Hdom_mem_p_rx3).
-    iDestruct ((big_sepM_union _ _) with "Hmem") as "(Hmem2 & p_rx3)";auto.
-    rewrite set_of_addr_union in Hdom_mem1.
-    2 : {
-      solve_NoDup 7.
-    }
     apply dom_union_inv_L in Hdom_mem1.
     2 : {
       apply set_of_addr_disj.
-      solve_NoDup 7.
+      solve_NoDup 8.
     }
-    destruct Hdom_mem1 as (mem4 & mem_p_rx2 &  -> & Hmem4_disj  & Hdom_mem2 & Hdom_mem_p_rx2).
-    iDestruct ((big_sepM_union _ _) with "Hmem2") as "(Hmem2 & p_rx2)";auto.
-    rewrite set_of_addr_union in Hdom_mem2.
-    2 : {
-      solve_NoDup 6.
-    }
-    apply dom_union_inv_L in Hdom_mem2.
-    2 : {
-      apply set_of_addr_disj.
-      solve_NoDup 6.
-    }
-    destruct Hdom_mem2 as (mem5 & mem_p_rx1 &  -> & Hmem5_disj  & Hdom_mem1 & Hdom_mem_p_rx1).
+    destruct Hdom_mem1 as (mem4 & mem_p_rx1 &  -> & Hmem4_disj  & Hdom_mem2 & Hdom_mem_p_rx1).
     iDestruct ((big_sepM_union _ _) with "Hmem2") as "(Hmem2 & p_rx1)";auto.
-    rewrite set_of_addr_union in Hdom_mem1.
-    2 : {
-      solve_NoDup 5.
-    }
-    apply dom_union_inv_L in Hdom_mem1.
-    2 : {
-      apply set_of_addr_disj.
-      solve_NoDup 5.
-    }
-    destruct Hdom_mem1 as (mem3 & mem_p_tx3 & -> & Hmem6_disj  & Hdom_mem2 & Hdom_mem_p_tx3).    
-    iDestruct ((big_sepM_union _ _) with "Hmem2") as "(Hmem2 & p_tx3)";auto.
     rewrite set_of_addr_union in Hdom_mem2.
     2 : {
-      solve_NoDup 4.
+      solve_NoDup 7.
     }
     apply dom_union_inv_L in Hdom_mem2.
     2 : {
       apply set_of_addr_disj.
-      solve_NoDup 4.
+      solve_NoDup 7.
     }
-    destruct Hdom_mem2 as (mem4 & mem_p_tx2 & -> & Hmem7_disj  & Hdom_mem2 & Hdom_mem_p_tx2).    
+    destruct Hdom_mem2 as (mem5 & mem_p_rx0 &  -> & Hmem5_disj  & Hdom_mem1 & Hdom_mem_p_rx0).
+    iDestruct ((big_sepM_union _ _) with "Hmem2") as "(Hmem2 & p_rx0)";auto.
+    rewrite set_of_addr_union in Hdom_mem1.
+    2 : {
+      solve_NoDup 6.
+    }
+    apply dom_union_inv_L in Hdom_mem1.
+    2 : {
+      apply set_of_addr_disj.
+      solve_NoDup 6.
+    }
+    destruct Hdom_mem1 as (mem3 & mem_p_tx2 & -> & Hmem6_disj  & Hdom_mem2 & Hdom_mem_p_tx2).
     iDestruct ((big_sepM_union _ _) with "Hmem2") as "(Hmem2 & p_tx2)";auto.
     rewrite set_of_addr_union in Hdom_mem2.
     2 : {
-      solve_NoDup 3.
+      solve_NoDup 5.
     }
     apply dom_union_inv_L in Hdom_mem2.
     2 : {
       apply set_of_addr_disj.
-      solve_NoDup 3.
+      solve_NoDup 5.
     }
-    destruct Hdom_mem2 as (mem5 & mem_p_tx1 & -> & Hmem8_disj  & Hdom_mem3 & Hdom_mem_p_tx1).    
+    destruct Hdom_mem2 as (mem4 & mem_p_tx1 & -> & Hmem7_disj  & Hdom_mem2 & Hdom_mem_p_tx1).
     iDestruct ((big_sepM_union _ _) with "Hmem2") as "(Hmem2 & p_tx1)";auto.
+    rewrite set_of_addr_union in Hdom_mem2.
+    2 : {
+      solve_NoDup 4.
+    }
+    apply dom_union_inv_L in Hdom_mem2.
+    2 : {
+      apply set_of_addr_disj.
+      solve_NoDup 4.
+    }
+    destruct Hdom_mem2 as (mem5 & mem_p_tx0 & -> & Hmem8_disj  & Hdom_mem3 & Hdom_mem_p_tx0).
+    iDestruct ((big_sepM_union _ _) with "Hmem2") as "(Hmem2 & p_tx0)";auto.
     
     subst p q r t.
     
@@ -497,143 +505,34 @@ Section mtms_adequacy.
 
     iAssert (trans.fresh_handles 1 valid_handles)%I with "[Hhpool Htrans Hretri]" as "Hp".
     {
-      destruct Htrans as [Htrans1 Htrans2].
-      rewrite <-Htrans1.
       unfold trans.fresh_handles.
       unfold get_hpool_gset.
       unfold get_fresh_handles.
       rewrite hpool_mapsto_eq /hpool_mapsto_def.
+      rewrite Htrans.
       simpl.
-      assert ((filter (λ (kv : Addr * option transaction), kv.2 = None) σ.2) = σ.2) as Heq.
-      {
-        rewrite map_eq_iff.
-        intros i.
-        rewrite map_filter_lookup.
-        rewrite map_Forall_lookup in Htrans2.
-        specialize (Htrans2 i).
-        destruct (σ.2 !! i) eqn:Heqn.
-        - rewrite Heqn.
-          simpl.
-          specialize (Htrans2 o Heqn).
-          rewrite Htrans2.
-          simpl.
-          reflexivity.
-        - rewrite Heqn.
-          reflexivity.
-      }
-      rewrite Heq.
-      assert ((dom σ.2 ∩ {[W0]}) = (dom σ.2)) as ->.
-      {
-        rewrite Htrans1.
-        set_solver +.
-      }
+      rewrite map_filter_singleton_True.
+      rewrite dom_singleton_L.
+      rewrite intersection_idemp_L.
       iFrame "Hhpool".
-      
+
       rewrite big_sepS_sep.
+      unfold get_trans_gmap.
+      unfold get_retri_gmap.
+      unfold get_transactions_gmap.
+      rewrite Htrans.
+      rewrite !map_fmap_singleton.
+      rewrite !big_sepM_singleton.
+      rewrite !big_sepS_singleton.
       iSplitL "Htrans".      
-      - unfold get_trans_gmap.
-        unfold get_transactions_gmap.
-        rewrite trans_mapsto_eq /trans_mapsto_def.
-        match goal with
-        | |- context G [?f <$> σ.2] => set g := f
-        end.
-        assert (∀ (m : gmap Addr (option transaction))
-                  (f : option transaction -> option meta_info), map_Forall (λ _ v, v = None) m -> (f None = None) -> (∀ i j, (f <$> m) !! i = Some j -> j = None)) as Heq'.
-        {
-          intros m f Hm Hf.
-          intros i j.
-          rewrite map_Forall_lookup in Hm.
-          specialize (Hm i).
-          rewrite lookup_fmap.
-          destruct (m !! i) eqn:Heqn.
-          - intros eq.
-            specialize (Hm o eq_refl).
-            rewrite Hm in eq.
-            simpl in eq.
-            rewrite Hf in eq.
-            inversion eq.
-            reflexivity.
-          - intros eq.
-            simpl in eq.
-            discriminate.
-        }
-        specialize (Heq' σ.2 g Htrans2).
-        feed specialize Heq'.
-        {
-          subst g.
-          simpl.
-          reflexivity.
-        }
-        simpl.
-        assert (map_Forall (λ (_ : Addr) (v : option (@meta_info rywu_vmconfig)), v = None) (g <$> σ.2)) as Htrans3.
-        {
-          intros i j He.
-          by apply (Heq' i).
-        }
-        pose proof (big_opM_dom (fun (y : finz.finz 2000000) => ghost_map_elem trans_gname y (DfracOwn (pos_to_Qp 1)) None) σ.2) as Hrew.
-        simpl in Hrew.
-        rewrite big_sepS_sep.
-        rewrite <-Hrew.
-        clear Hrew.
-        rewrite big_opM_fmap.
-        rewrite big_op.big_opM_unseal /big_op.big_opM_def.        
-        rewrite (big_opL_ext (λ _, uncurry
-                                     (λ (k : Addr) (_ : option transaction),
-                                      (k ↪[trans_gname] None)%I))
-                             (λ _, uncurry (λ (k : Addr) (y : option transaction),
-                                            (k ↪[trans_gname] g y)%I))
-                             (map_to_list σ.2)).
-        iFrame "Htrans".
-        {
-          iPureIntro.
-          rewrite Htrans1.
-          intro.
-          set_solver +.
-        }
-        intros k (y1 & y2) eq'.
-        simpl. subst g.
-        assert (y2 = None) as ->.
-        {
-          rewrite map_Forall_to_list in Htrans2.
-          apply (Forall_lookup_1 _ _ k (pair y1 y2)) in Htrans2; last done.
-          simpl in Htrans2.
-          assumption.
-        }
-        reflexivity.
-      - unfold get_retri_gmap.
-        unfold get_transactions_gmap.
-        rewrite retri_mapsto_eq /retri_mapsto_def.
-        match goal with
-        | |- context G [?f <$> σ.2] => set g := f
-        end.
-        rewrite big_opM_fmap.
-        simpl.
-        set f := (λ k v, (k ↪[retri_gname] g v)%I).
-        pose f' := (λ k _, f k None).
-        rewrite (big_opM_ext f
-                             (λ k v, f' (option transaction) k v)
-                             σ.2).
-        2: {
-          intros k x G.
-          subst f f' g. simpl.
-          rewrite map_Forall_lookup in Htrans2.
-          specialize (Htrans2 k x G).
-          rewrite Htrans2 //=.
-        }
-        subst f'. simpl.
-        subst f. simpl.
-        rewrite big_opM_dom.
-        rewrite big_sepS_sep.
-        iFrame "Hretri".
-        {
-          iPureIntro.
-          rewrite Htrans1.
-          intro.
-          set_solver +.
-        }
+      rewrite trans_mapsto_eq /trans_mapsto_def /=.
+      iFrame. done.
+      rewrite retri_mapsto_eq /retri_mapsto_def /=.
+      iFrame. done.
+      done.
     }
     
-    iDestruct (big_sepM_subseteq _ (get_access_gmap σ) {[V0 := (to_dfrac_agree (DfracOwn 1) ({[tpa addr; p_prog1; p_tx1]})); V1 := (to_dfrac_agree (DfracOwn 1) ({[p_prog2; p_tx2; p_rx2]})); V2 := (to_dfrac_agree (DfracOwn 1) ({[p_tx3;p_rx3;p_prog3]}))]} with "Haccess") as "access"; eauto.
+    iDestruct (big_sepM_subseteq _ (get_access_gmap σ) {[V0 := (to_dfrac_agree (DfracOwn 1) ({[p_share; p_prog0; p_tx0]})); V1 := (to_dfrac_agree (DfracOwn 1) ({[p_prog1; p_tx1; p_rx1]})); V2 := (to_dfrac_agree (DfracOwn 1) ({[p_tx2;p_rx2;p_prog2]}))]} with "Haccess") as "access"; eauto.
     {
       apply access_layout_get_access_gmap.
       assumption.
@@ -665,7 +564,7 @@ Section mtms_adequacy.
     iEval (rewrite big_sepM_singleton) in "access".
     iDestruct "access" as "(access1 & access2 & access3)".
     
-    iDestruct (big_sepM_subseteq _ (get_excl_gmap σ) {[p_rx1 := true; p_rx2 := true; p_rx3 := true; p_tx3 := true; p_prog3 := true; tpa addr := true]} with "Hexcl") as "excl"; eauto.
+    iDestruct (big_sepM_subseteq _ (get_excl_gmap σ) {[p_rx0 := true; p_rx1 := true; p_rx2 := true; p_tx2 := true; p_prog2 := true; p_share := true]} with "Hexcl") as "excl"; eauto.
     {
       apply excl_layout_get_excl_gmap.
       assumption.
@@ -674,25 +573,36 @@ Section mtms_adequacy.
     match goal with
     | |- context G [delete _ ?p] => set P := p
     end.
-    assert (delete p_rx1 P = P) as ->.
+    assert (delete p_rx0 P = P) as ->.
     {
       subst P.      
-      clear -Hnodup_p.      
       apply delete_notin.
       rewrite <-not_elem_of_dom.      
       rewrite !dom_insert_L.
       rewrite dom_empty_L.
       rewrite union_empty_r.      
-      rewrite !elem_of_union.      
-      rewrite !elem_of_singleton.
-      intros contra.      
+      solve_NoDup_pre.
       solve_NoDup_pre'.
-      solve_NoDup_pre'' 6 7.
+      solve_NoDup_pre'' 7 8.
+      solve_NoDup 7.
+    }
+    subst P.
+    iEval (rewrite big_opM_insert_delete) in "excl".
+    match goal with
+    | |- context G [delete _ ?p] => set P := p
+    end.
+    assert (delete p_rx1 P = P) as ->.
+    {
+      subst P.
+      apply delete_notin.
+      rewrite <-not_elem_of_dom.
+      rewrite !dom_insert_L.
+      rewrite dom_empty_L.
+      rewrite union_empty_r.      
+      solve_NoDup_pre.
       solve_NoDup_pre'.
-      solve_NoDup_pre'' 6 8.
-      solve_NoDup_pre'' 5 6.
-      solve_NoDup_pre'' 2 6.
-      solve_NoDup_pre'' 6 9.
+      solve_NoDup_pre'' 8 9.
+      solve_NoDup 8.
     }
     subst P.
     iEval (rewrite big_opM_insert_delete) in "excl".
@@ -702,75 +612,44 @@ Section mtms_adequacy.
     assert (delete p_rx2 P = P) as ->.
     {
       subst P.
-      clear -Hnodup_p.      
       apply delete_notin.
       rewrite <-not_elem_of_dom.
       rewrite !dom_insert_L.
       rewrite dom_empty_L.
       rewrite union_empty_r.      
-      rewrite !elem_of_union.
-      rewrite !elem_of_singleton.
-      intros contra.
+      solve_NoDup_pre.
       solve_NoDup_pre'.
-      solve_NoDup_pre'' 7 8.
-      solve_NoDup_pre'.
-      solve_NoDup_pre'' 5 7.
-      solve_NoDup_pre'' 2 7.
-      solve_NoDup_pre'' 7 9.
-    }
-    subst P.
-    iEval (rewrite big_opM_insert_delete) in "excl".
-    match goal with
-    | |- context G [delete _ ?p] => set P := p
-    end.
-    assert (delete p_rx3 P = P) as ->.
-    {
-      subst P.
-      clear -Hnodup_p.      
-      apply delete_notin.
-      rewrite <-not_elem_of_dom.
-      rewrite !dom_insert_L.
-      rewrite dom_empty_L.
-      rewrite union_empty_r.      
-      rewrite !elem_of_union.
-      rewrite !elem_of_singleton.
-      intros contra.
-      solve_NoDup_pre'.
-      solve_NoDup_pre'' 5 8.
+      solve_NoDup_pre'' 6 9.
       destruct eq as [-> | ->].
-      solve_NoDup_pre'' 2 8.
-      solve_NoDup_pre'' 8 9.
+      solve_NoDup_pre'' 2 9.
+      solve_NoDup_pre'' 3 9.
     }
     subst P.
     iEval (rewrite big_opM_insert_delete) in "excl".
     match goal with
     | |- context G [delete _ ?p] => set P := p
     end.
-    assert (delete p_tx3 P = P) as ->.
+    assert (delete p_tx2 P = P) as ->.
     {
       subst P.
-      clear -Hnodup_p.      
       apply delete_notin.
       rewrite <-not_elem_of_dom.
       rewrite !dom_insert_L.
       rewrite dom_empty_L.
       rewrite union_empty_r.
-      rewrite !elem_of_union.
-      rewrite !elem_of_singleton.
-      intros contra.
+      solve_NoDup_pre.
       destruct contra as [-> | ->].
-      solve_NoDup_pre'' 2 5.
-      solve_NoDup_pre'' 5 9.
+      solve_NoDup_pre'' 2 6.
+      solve_NoDup_pre'' 3 6.
     }
     subst P.
     iEval (rewrite big_opM_insert_delete) in "excl".
     match goal with
     | |- context G [delete _ ?p] => set P := p
     end.
-    assert (delete p_prog3 P = P) as ->.
+    assert (delete p_prog2 P = P) as ->.
     {
       subst P.
-      clear -Hnodup_p.      
       apply delete_notin.
       rewrite <-not_elem_of_dom.
       rewrite !dom_insert_L.
@@ -778,14 +657,14 @@ Section mtms_adequacy.
       rewrite union_empty_r.
       rewrite !elem_of_singleton.
       intros ->.
-      solve_NoDup_pre'' 2 9.
+      solve_NoDup_pre'' 2 3.
     }
     subst P.
       
     iEval (rewrite big_sepM_singleton) in "excl".
     iDestruct "excl" as "(excl1 & excl2 & excl3 & excl4 & excl5 & excl6)".
 
-    iDestruct (big_sepM_subseteq _ (get_own_gmap σ) {[p_rx1 := None; p_rx2 := None; p_rx3 := None; p_tx3 := None; p_prog3 := Some V2; tpa addr := Some V0]} with "Hown") as "own"; eauto.
+    iDestruct (big_sepM_subseteq _ (get_own_gmap σ) {[p_rx0 := None; p_rx1 := None; p_rx2 := None; p_tx2 := None; p_prog2 := Some V2; p_share := Some V0]} with "Hown") as "own"; eauto.
     {
       apply own_layout_get_own_gmap.
       assumption.      
@@ -794,25 +673,36 @@ Section mtms_adequacy.
     match goal with
     | |- context G [delete _ ?p] => set P := p
     end.
-    assert (delete p_rx1 P = P) as ->.
+    assert (delete p_rx0 P = P) as ->.
     {
       subst P.
-      clear -Hnodup_p.      
       apply delete_notin.
       rewrite <-not_elem_of_dom.
       rewrite !dom_insert_L.
       rewrite dom_empty_L.
       rewrite union_empty_r.
-      rewrite !elem_of_union.
-      rewrite !elem_of_singleton.
-      intros contra.
+      solve_NoDup_pre.
       solve_NoDup_pre'.
-      solve_NoDup_pre'' 6 7.
+      solve_NoDup_pre'' 7 8.
+      solve_NoDup 7.
+    }
+    subst P.
+    iEval (rewrite big_opM_insert_delete) in "own".
+    match goal with
+    | |- context G [delete _ ?p] => set P := p
+    end.
+    assert (delete p_rx1 P = P) as ->.
+    {
+      subst P.
+      apply delete_notin.
+      rewrite <-not_elem_of_dom.
+      rewrite !dom_insert_L.
+      rewrite dom_empty_L.
+      rewrite union_empty_r.
+      solve_NoDup_pre.
       solve_NoDup_pre'.
-      solve_NoDup_pre'' 6 8.
-      solve_NoDup_pre'' 5 6.
-      solve_NoDup_pre'' 2 6.
-      solve_NoDup_pre'' 6 9.
+      solve_NoDup_pre'' 8 9.
+      solve_NoDup 8.
     }
     subst P.
     iEval (rewrite big_opM_insert_delete) in "own".
@@ -822,84 +712,45 @@ Section mtms_adequacy.
     assert (delete p_rx2 P = P) as ->.
     {
       subst P.
-      clear -Hnodup_p.      
       apply delete_notin.
       rewrite <-not_elem_of_dom.
       rewrite !dom_insert_L.
       rewrite dom_empty_L.
       rewrite union_empty_r.
-      rewrite !elem_of_union.
-      rewrite !elem_of_singleton.
-      intros contra.
+      solve_NoDup_pre.
       solve_NoDup_pre'.
-      solve_NoDup_pre'' 7 8.
-      solve_NoDup_pre'.
-      solve_NoDup_pre'' 5 7.
-      solve_NoDup_pre'' 2 7.
-      solve_NoDup_pre'' 7 9.
+      solve_NoDup_pre'' 6 9.
+      solve_NoDup 9.
     }
     subst P.
     iEval (rewrite big_opM_insert_delete) in "own".
     match goal with
     | |- context G [delete _ ?p] => set P := p
     end.
-    assert (delete p_rx3 P = P) as ->.
+    assert (delete p_tx2 P = P) as ->.
     {
       subst P.
-      clear -Hnodup_p.      
       apply delete_notin.
       rewrite <-not_elem_of_dom.
       rewrite !dom_insert_L.
       rewrite dom_empty_L.
       rewrite union_empty_r.
-      rewrite !elem_of_union.
-      rewrite !elem_of_singleton.
-      intros contra.
-      solve_NoDup_pre'.
-      solve_NoDup_pre'' 5 8.
-      solve_NoDup_pre'.
-      solve_NoDup_pre'' 2 8.
-      solve_NoDup_pre'' 8 9.
+      solve_NoDup 6.
     }
     subst P.
     iEval (rewrite big_opM_insert_delete) in "own".
     match goal with
     | |- context G [delete _ ?p] => set P := p
     end.
-    assert (delete p_tx3 P = P) as ->.
+    assert (delete p_prog2 P = P) as ->.
     {
       subst P.
-      clear -Hnodup_p.      
       apply delete_notin.
       rewrite <-not_elem_of_dom.
       rewrite !dom_insert_L.
       rewrite dom_empty_L.
       rewrite union_empty_r.
-      rewrite !elem_of_union.
-      rewrite !elem_of_singleton.  
-      intros contra.
-      solve_NoDup_pre'.
-      solve_NoDup_pre'' 2 5.
-      solve_NoDup_pre'' 5 9.
-    }
-    subst P.
-    iEval (rewrite big_opM_insert_delete) in "own".
-    match goal with
-    | |- context G [delete _ ?p] => set P := p
-    end.
-    assert (delete p_prog3 P = P) as ->.
-    {
-      subst P.
-      clear -Hnodup_p.      
-      apply delete_notin.
-      rewrite <-not_elem_of_dom.
-      rewrite !dom_insert_L.
-      rewrite dom_empty_L.
-      rewrite union_empty_r.
-      rewrite !elem_of_singleton.  
-      intros contra.
-      solve_NoDup_pre'.
-      solve_NoDup_pre'' 2 5.
+      solve_NoDup 3.
     }
     subst P.
     iEval (rewrite big_sepM_singleton) in "own".
@@ -917,11 +768,11 @@ Section mtms_adequacy.
     (* allocate VMProps *)
     set pgt := (get_page_table σ).    
     iExists [True%I;
-      (R0 @@ V0 ->r run_I ∗ R1 @@ V0 ->r encode_vmid V1 ∗ addr ->a two  ∗ (∃ (wh : Addr), (∃ (β : lang.mem), wh ->t (V0, V1, {[tpa addr]}, Sharing) ∗
-                                                                                    wh ->re false ∗ RX_state@V1 := Some (of_imm one, V0) ∗ RX@V1:=p_rx2 ∗ memory_page p_rx2 β ∗ ⌜β !! (of_imm rxbase) = Some wh⌝) ∗
-                    VMProp V0 ((R0 @@ V0 ->r yield_I ∗ R1 @@ V0 ->r encode_vmid V1 ∗ addr ->a four ∗ wh ->t (V0, V1, {[tpa addr]}, Sharing) ∗ RX@V1:=p_rx2 ∗ RX_state@V1 := None ∗ (∃ mem_rx, memory_page p_rx2 mem_rx)) ∗
+      (R0 @@ V0 ->r run_I ∗ R1 @@ V0 ->r encode_vmid V1 ∗ addr ->a two  ∗ (∃ (wh : Addr), (∃ (β : lang.mem), wh ->t (V0, V1, {[p_share]}, Sharing) ∗
+                                                                                    wh ->re false ∗ RX_state@V1 := Some (of_imm one, V0) ∗ RX@V1:=p_rx1 ∗ memory_page p_rx1 β ∗ ⌜β !! (of_imm i_prx1) = Some wh⌝) ∗
+                    VMProp V0 ((R0 @@ V0 ->r yield_I ∗ R1 @@ V0 ->r encode_vmid V1 ∗ addr ->a four ∗ wh ->t (V0, V1, {[p_share]}, Sharing) ∗ RX@V1:=p_rx1 ∗ RX_state@V1 := None ∗ (∃ mem_rx, memory_page p_rx1 mem_rx)) ∗
                                  VMProp V1 False%I (1/2)%Qp) (1/2)%Qp))%I;
-      (vmprop_unknown V2 (* p_tx p_rx  *) ∅)].
+      (vmprop_unknown V2 mtms_slice_trans mtms_slice_rxs ∅)].
     iSimpl.
     iSplit; first done.
 
@@ -930,138 +781,100 @@ Section mtms_adequacy.
     iFrame.
     rewrite /inv_trans_wellformed /inv_trans_wellformed'.
     rewrite /inv_trans_pgt_consistent /inv_trans_pgt_consistent'.
-    destruct Htrans as [Hdom_trans Hempty_trans].
+    rewrite Htrans.
     repeat iSplit.
     done.
     {
       rewrite /inv_trans_pg_num_ub.
       iPureIntro.
-      eapply (map_Forall_impl (K:=Word) (M:= gmap Word)).
-      apply Hempty_trans.
-      intros h tran Hnone.
-      simpl in Hnone.
-      subst tran.
-      done.
+      rewrite map_Forall_singleton //.
     }
     {
       rewrite /inv_trans_sndr_rcvr_neq.
       iPureIntro.
-      eapply (map_Forall_impl (K:=Word) (M:= gmap Word)).
-      apply Hempty_trans.
-      intros h tran Hnone.
-      simpl in Hnone.
-      subst tran.
-      done.
+      rewrite map_Forall_singleton //.
     }
     {
       rewrite /inv_finite_handles.
       iPureIntro.
-      rewrite -Hdom_trans //.
+      rewrite dom_singleton_L //.
     }
     {
       iPureIntro.
-      eapply (map_Forall_impl (K:=Word) (M:= gmap Word)).
-      apply Hempty_trans.
-      intros h tran Hnone.
-      simpl in Hnone.
-      subst tran.
-      done.
+      rewrite /inv_trans_ps_disj /inv_trans_ps_disj'.
+      rewrite Htrans.
+      rewrite map_Forall_singleton //.
     }
     {
       iPureIntro.
-      intros ? ? Hlk.
-      specialize (Hempty_trans _ _ Hlk).
-      simpl in Hempty_trans.
-      subst x. done.
+      rewrite map_Forall_singleton //.
     }
 
     iIntros "(VMProp0 & VMProp1 & VMProp2 & _)".
-    rewrite /scheduled /machine.scheduler //= /scheduler Hcur //=.
+    rewrite /scheduled /machine.scheduler /= /scheduler Hcur /=.
       
     iDestruct (VMProp_split with "VMProp1") as "[VMProp1_half VMProp1_half']".
     iDestruct (VMProp_split with "VMProp2") as "[VMProp2_half VMProp2_half']".
     
-    pose proof (@access_split rywu_vmconfig irisΣ VMG 1 V2) as Hsplit.
+    pose proof (@access_split mtms_vmconfig irisΣ VMG 1 V2) as Hsplit.
     rewrite access_mapsto_eq /access_mapsto_def in Hsplit.
     (* iDestruct "access3" as "(access3 & access3')". *)
-    iAssert ((V2, RX) ↪[ mb_gname ]□ p_rx3 ∗ (V2, RX) ↪[ mb_gname ]□ p_rx3)%I with "[mb2RX]" as "(mb2RX & mb2RX')".
+    iAssert ((V2, RX) ↪[ mb_gname ]□ p_rx2 ∗ (V2, RX) ↪[ mb_gname ]□ p_rx2)%I with "[mb2RX]" as "(mb2RX & mb2RX')".
     {
       iDestruct "mb2RX" as "#mb2RX".
       iFrame "mb2RX".
     }
     
-    iSplitL "PCz R0z R1z R2z R3z R4z R5z mem_p_prog1 p_tx1 mem_p Hp VMProp0 VMProp1_half' VMProp2_half' mb0RX mb1RX RX0St RX1St RX2St p_rx1 p_rx2 p_rx3 mb0TX mb2RX access1 excl1 excl2 excl6 own1 own2 own6".
+    iSplitL "PCz R0z R1z R2z R3z R4z R5z mem_p_prog0 p_tx0 mem_p Hp VMProp0 VMProp1_half' VMProp2_half' mb0RX mb1RX RX0St RX1St RX2St p_rx0 p_rx1 p_rx2 mb0TX mb2RX access1 excl1 excl2 excl6 own1 own2 own6".
     iIntros "_".
-    iDestruct (lending_machine0 p_prog1 p_tx1 p_prog3 p_tx3 p_rx1 p_rx2 p_rx3 addr txbase rxbase with "[-]") as "HWP".
+
+    iApply (wp_mono _ _ _ (λ m,  ⌜m = HaltI⌝ ∗
+                 addr ->a four ∗
+            V0 -@A> {[p_share; p_prog0; p_tx0]} ∗ TX@V0:=p_tx0 ∗
+                 PC @@ V0 ->r ((of_pid p_prog0) ^+ (length (mtms_program0 addr i_ptx0)))%f)%I).
+    intros.
+    iIntros "[$ _]".
+    
+    iApply (mtms_machine0 p_prog0 p_prog1 p_prog2 p_tx0 p_rx0 p_tx1 p_rx1 p_tx2 p_rx2 p_share Hps_nd with "[-]").  
     {
-      assumption.
+      exact Heq_pshare.
     }
-    {
-      assumption.
-    }
-    {
-      assumption.
-    }
-    {
-      solve_NoDup 0.
-    }
-    {
-      clear -Hnodup_p.
-      intros <-.
-      solve_NoDup_pre'' 6 9.
-    }
-    {
-      clear -Hnodup_p.
-      intros <-.
-      solve_NoDup_pre'' 0 9.
-    }
-    {
-      clear -Hnodup_p.
-      intros <-.
-      solve_NoDup_pre'' 3 9.
-    }
-    {
-      clear -Hnodup_p.
-      intros <-.
-      solve_NoDup_pre'' 3 6.
-    }
+    assumption.
+    exact Heq_prx1.
+    program_in_seq.
+    iSplitL "mem_p_prog0".
     {      
-      program_in_seq.     
-    }
-    {
-      iSplitL "mem_p_prog1".
-      {      
-        unfold program.
-        iEval (rewrite big_opM_map_to_list) in "mem_p_prog1".
-        rewrite big_sepL2_alt.
-        iSplitR "mem_p_prog1".
-        {
-          simpl.
-          by iPureIntro.
-        }
-        {
-          rewrite mem_mapsto_eq /mem_mapsto_def.
-          assert (mem_p_prog1 ⊆ σ.1.2) as Hsubseteq.
-          {
-            rewrite Hunion_mem'.
-            apply map_union_subseteq_r'.
-            assumption.
-            apply map_union_subseteq_r'.
-            assumption.
-            done.
-          }
-          iApply (memory_list_gmap _ _ _ mem_p_prog1 σ).
-          - rewrite fst_zip.
-            + apply finz_seq_NoDup'.
-              simpl.
-              pose proof (last_addr_in_bound p_prog1).
-              solve_finz.
-            + simpl.
-              lia.
-          - apply HmemH1; done.
-          - by iFrame.
-        }
+      unfold program.
+      iEval (rewrite big_opM_map_to_list) in "mem_p_prog0".
+      rewrite big_sepL2_alt.
+      iSplitR "mem_p_prog0".
+      {
+        simpl.
+        by iPureIntro.
       }
+      {
+        rewrite mem_mapsto_eq /mem_mapsto_def.
+        assert (mem_p_prog0 ⊆ σ.1.2) as Hsubseteq.
+        {
+          rewrite Hunion_mem'.
+          apply map_union_subseteq_r'.
+          assumption.
+          apply map_union_subseteq_r'.
+          assumption.
+          done.
+        }
+
+        iApply (memory_list_gmap p_prog0 (mtms_program0 addr i_ptx0) _ mem_p_prog0 with "mem_p_prog0").
+        - rewrite fst_zip.
+          + apply finz_seq_NoDup'.
+            simpl.
+            pose proof (last_addr_in_bound p_prog0).
+            solve_finz.
+          + simpl.
+            lia.
+        - apply HmemH1; done.
+      }
+    }
       iSplitL "mem_p".
       {
         rewrite mem_mapsto_eq /mem_mapsto_def.
@@ -1076,10 +889,12 @@ Section mtms_adequacy.
           assumption.
           done.
         }
-        assert (of_imm addr ∈ set_of_addr {[tpa addr]}) as H.
+        assert (of_imm addr ∈ set_of_addr {[p_share]}) as H.
         {
-          apply elem_of_set_of_addr with (tpa addr).
-          apply elem_of_addr_of_page_tpa.
+          apply elem_of_set_of_addr with (p_share).
+          rewrite -Heq_pshare.
+          apply elem_of_addr_of_page_iff.
+          rewrite to_pid_aligned_eq //.
           set_solver +.
         }
         rewrite <-Hdom_mem_p in H.
@@ -1090,13 +905,11 @@ Section mtms_adequacy.
         iExists waddr.
         iFrame.        
       }
-      iSplitL "p_tx1".
+      iSplitL "p_tx0".
       {
         unfold memory_page.
-        iExists mem_p_tx1. iSplit. rewrite Hdom_mem_p_tx1. iPureIntro.
-        rewrite set_of_addr_singleton.
-        rewrite to_pid_aligned_eq.
-        reflexivity.
+        iExists mem_p_tx0. iSplit. rewrite Hdom_mem_p_tx0. iPureIntro.
+        rewrite set_of_addr_singleton //.
         rewrite mem_mapsto_eq /mem_mapsto_def /=.
         iFrame.
       }
@@ -1104,7 +917,6 @@ Section mtms_adequacy.
       iFrame "RX0St RX1St RX2St".
       unfold rx_page.
       rewrite mb_mapsto_eq /mb_mapsto_def /=.
-      rewrite to_pid_aligned_eq.
       iFrame "mb0TX".
       iFrame "PCz".
       rewrite access_mapsto_eq /access_mapsto_def /=.
@@ -1116,10 +928,7 @@ Section mtms_adequacy.
       }
       iSplitL "access1".
       {
-        assert ({[tpa addr; p_prog1; p_tx1]} = {[tpa addr]} ∪ {[p_prog1; p_tx1]}) as ->.
-        {
-          set_solver +.
-        }
+        rewrite /to_frac_agree.
         iFrame.
       }      
       iSplitL "R0z".
@@ -1140,91 +949,54 @@ Section mtms_adequacy.
       iFrame "Hp".
       iFrame.      
 
-      iSplitL "p_rx1 excl1 own1".      
-      iSplitR "p_rx1".
+      iSplitL "p_rx0 excl1 own1".
+      iSplitR "p_rx0".
       rewrite excl_mapsto_eq own_mapsto_eq /excl_mapsto_def /own_mapsto_def /=.
       iFrame.
       unfold memory_page.
+      iExists mem_p_rx0. iSplit. rewrite Hdom_mem_p_rx0. iPureIntro.
+      apply set_of_addr_singleton.
+      rewrite mem_mapsto_eq /mem_mapsto_def /=.
+      iFrame "p_rx0".
+      iSplitL "p_rx1 excl2 own2".
       iExists mem_p_rx1. iSplit. rewrite Hdom_mem_p_rx1. iPureIntro.
       apply set_of_addr_singleton.
       rewrite mem_mapsto_eq /mem_mapsto_def /=.
       iFrame "p_rx1".
-      iSplitL "p_rx2 excl2 own2".      
-      iSplitR "p_rx2".
-      rewrite excl_mapsto_eq own_mapsto_eq /excl_mapsto_def /own_mapsto_def /=.
-      iFrame.
       unfold memory_page.
       iExists mem_p_rx2. iSplit. rewrite Hdom_mem_p_rx2. iPureIntro.
       apply set_of_addr_singleton.
       rewrite mem_mapsto_eq /mem_mapsto_def /=.
       iFrame "p_rx2".
-
-      unfold memory_page.
-      iExists mem_p_rx3. iSplit. rewrite Hdom_mem_p_rx3. iPureIntro.
-      apply set_of_addr_singleton.
-      rewrite mem_mapsto_eq /mem_mapsto_def /=.
-      iFrame "p_rx3".
-    }
     
-    iApply (wp_mono with "HWP").
-    intros k.
-    simpl.
-    iIntros "[$ _]".
+    iSplitL "VMProp1_half PC1 R01 R11 R21 R31 R41 R51 mem_p_prog1 p_tx1 mb1TX access2".
 
-    iSplitL "VMProp1_half PC1 R01 R11 R21 R31 R41 R51 mem_p_prog2 p_tx2 mb1TX access2".
-    iApply (lending_machine1 p_prog2 p_tx2 p_rx2 addr rxbase).
+    iAssert ((VMProp_holds V1 (1 / 2) -∗ WP ExecI @ V1 {{ _, False }}) -∗
+            VMProp_holds 1 (1 / 2) -∗ WP ExecI @ 1 {{ _, False }})%I as "WP".
     {
-      assumption.
+      iIntros "H".
+      simpl.
+      iApply "H".
+    }
+    iApply "WP".
+    iApply (mtms_machine1 p_prog0 p_prog1 p_prog2 p_tx0 p_rx0 p_tx1 p_rx1 p_tx2 p_rx2 p_share Hps_nd with "[-]").
+    {
+      exact Heq_pshare.
     }
     {
-      assumption.
-    }
-    {      
-      clear -Hnodup_p.
-      intros contra.
-      rewrite !elem_of_union in contra.
-      rewrite !elem_of_singleton in contra.
-      destruct contra as [[H | H] | H]; subst.
-      solve_NoDup_pre'' 1 9.
-      solve_NoDup_pre'' 1 4.
-      solve_NoDup_pre'' 1 7.
-    }
-    {
-      clear -Hnodup_p.
-      intros contra.
-      subst.
-      solve_NoDup_pre'' 7 9.
-    }
-    {
-      clear -Hnodup_p.
-      intros contra.
-      subst.
-      solve_NoDup_pre'' 1 9.
-    }
-    {
-      clear -Hnodup_p.
-      intros contra.
-      subst.
-      solve_NoDup_pre'' 4 9.
-    }
-    {
-      clear -Hnodup_p.
-      intros contra.
-      subst.
-      solve_NoDup_pre'' 4 7.
+      exact Heq_prx1.
     }
     {
       program_in_seq.
     }
-    iFrame.        
-    iSplitL "mem_p_prog2".
+    iSplitL "mem_p_prog1".
     unfold program.
-    iEval (rewrite big_opM_map_to_list) in "mem_p_prog2".
+    iEval (rewrite big_opM_map_to_list) in "mem_p_prog1".
     rewrite big_sepL2_alt.
     iSplit; first done.
     rewrite mem_mapsto_eq /mem_mapsto_def.    
     {
-      assert (mem_p_prog2 ⊆ σ.1.2) as Hsubseteq.
+      assert (mem_p_prog1 ⊆ σ.1.2) as Hsubseteq.
       {
         rewrite Hunion_mem'.
         apply map_union_subseteq_r'.
@@ -1234,24 +1006,22 @@ Section mtms_adequacy.
         assumption.
         done.
       }
-      iApply (memory_list_gmap _ _ _ mem_p_prog2 σ).
+      iApply (memory_list_gmap _ _ _ mem_p_prog1).
       - rewrite fst_zip.
         + apply finz_seq_NoDup'.
           simpl.
-          pose proof (last_addr_in_bound p_prog2).
+          pose proof (last_addr_in_bound p_prog1).
           solve_finz.
         + simpl.
           lia.
       - apply HmemH2; done.
       - by iFrame.
     }
-    iSplitL "p_tx2".
+    iSplitL "p_tx1".
     {
       unfold memory_page.
-      iExists mem_p_tx2. iSplit. rewrite Hdom_mem_p_tx2. iPureIntro.
-      rewrite set_of_addr_singleton.
-      rewrite to_pid_aligned_eq.
-      reflexivity.
+      iExists mem_p_tx1. iSplit. rewrite Hdom_mem_p_tx1. iPureIntro.
+      rewrite set_of_addr_singleton //.
       rewrite mem_mapsto_eq /mem_mapsto_def /=.
       iFrame.
     }
@@ -1260,17 +1030,15 @@ Section mtms_adequacy.
     {
       rewrite access_mapsto_eq /access_mapsto_def.
       simpl.
-      rewrite !to_pid_aligned_eq.
       iFrame "access2".
     }
     
     iSplitL "mb1TX".
     {
       rewrite mb_mapsto_eq /mb_mapsto_def /=.
-      rewrite to_pid_aligned_eq.
       iFrame.
     }
-
+    iFrame "PC1".
     iSplitL "R01".
     iExists r0__.
     iFrame.
@@ -1286,129 +1054,165 @@ Section mtms_adequacy.
     iSplitL "R41".
     iExists r4__.
     iFrame.
+    iSplitL "R51".
     iExists r5__.
     iFrame.
-
+    iFrame "VMProp1_half".
+    
     iSplitR ""; last done.
-    iApply (mtms_ftlr p_prog3 p_tx3 p_rx3 with "[-] []").
-    2: { iPureIntro. cbn. done. }
-    { rewrite /mtms_interp_access /interp_access.
-      iSplitL "Hreg2".
-      iExists (get_reg_files σ !!! V2).
-      unfold get_reg_gmap_vm.
-      iSplit.
-      iPureIntro.
-      unfold base_extra.is_total_gmap.
-      apply Htotal_reg.
+    iAssert ((VMProp_holds V2 (1 / 2) -∗ WP ExecI @ V2 {{ _, True }}) -∗
+            VMProp_holds 2 (1 / 2) -∗ WP ExecI @ 2 {{ _, True }})%I as "WP".
+    {
+      iIntros "H".
       simpl.
-      {
-        set g := (λ p0 : reg_name * Addr, (p0.1, 2%fin, p0.2)).
-        unfold V2.
-        simpl.
-        set l := (σ.1.1.1.1.1 !!! 2%fin).
-        iEval (rewrite big_opM_map_to_list) in "Hreg2".
-        rewrite map_to_list_to_map.
-        rewrite big_opL_fmap.
-        subst g.
-        simpl.
-        rewrite big_opM_map_to_list.
-        iFrame "Hreg2".
-        subst g.
-        apply NoDup_fmap_fst.
-        intros [x1 x2] y1 y2 Hh Hh'.
-        rewrite elem_of_list_In in Hh.
-        rewrite elem_of_list_In in Hh'.
-        rewrite in_map_iff in Hh.
-        rewrite in_map_iff in Hh'.
-        destruct Hh as [(x & x') [Hheq Hh]].
-        destruct Hh' as [(t & t') [Hh'eq Hh']].
-        simpl in Hheq.
-        simpl in Hh'eq.
-        inversion Hheq.
-        inversion Hh'eq.
-        simplify_eq.
-        clear Hheq Hh'eq.
-        rewrite <-elem_of_list_In in Hh.
-        rewrite <-elem_of_list_In in Hh'.
-        apply map_to_list_unique with l x1; auto.
-        apply NoDup_fmap_2.
-        intros a b abeq.
-        inversion abeq.
-        destruct a, b; simpl in *.
-        by simplify_eq.
-        apply NoDup_map_to_list.
-      }
-      iFrame "VMProp2_half".
-      rewrite difference_empty_L.
-      unfold transaction_pagetable_entries_owned.
-      unfold retrieved_transaction_owned.
-      unfold big_sepFM. simpl.
-      rewrite map_filter_empty.
-      rewrite !big_sepM_empty.
-      assert (({[p_prog3; p_tx3; p_rx3]} ∖ {[p_rx3; p_tx3]}) = {[p_prog3]}) as ->.
-      {
-        rewrite !difference_union_distr_l_L.        
-        rewrite difference_disjoint_L.
-        assert ({[p_tx3]} ∖ {[p_rx3; p_tx3]} = ∅) as ->.
-        { set_solver +. }
-        assert ({[p_rx3]} ∖ {[p_rx3; p_tx3]} = ∅) as ->.
-        { set_solver +. }
-        set_solver +.
-        apply disjoint_singleton_l.
-        intros contra.
-        rewrite elem_of_union in contra.
-        rewrite !elem_of_singleton in contra.
-        solve_NoDup_pre'.
-        solve_NoDup_pre'' 2 8.
-        solve_NoDup_pre'' 2 5.
-      }
-      unfold pagetable_entries_excl_owned.
-      unfold logrel.pgt.
-      rewrite !big_sepS_singleton.
-      unfold tx_page.
-      iSplitL "mb2TX p_tx3 excl4 own4".
-      iSplitR "p_tx3".      
-      rewrite mb_mapsto_eq /mb_mapsto_def.
-      rewrite excl_mapsto_eq own_mapsto_eq /excl_mapsto_def /own_mapsto_def.
-      iFrame.
-      iExists mem_p_tx3. unfold memory_page. iSplit. iPureIntro.
-      rewrite Hdom_mem_p_tx3.
-      apply set_of_addr_singleton.
-      rewrite mem_mapsto_eq /mem_mapsto_def.
-      iFrame "p_tx3".
-      rewrite access_mapsto_eq /access_mapsto_def /=.
-      assert ({[p_tx3; p_rx3; p_prog3]} = {[p_prog3; p_tx3; p_rx3]}) as -> by set_solver +.
-      iFrame "access3".
-      unfold rx_page.
-
-      iSplitL "mb2RX' excl3 own3".
-      {
-        rewrite excl_mapsto_eq /excl_mapsto_def.
-        rewrite own_mapsto_eq /own_mapsto_def.
-        rewrite mb_mapsto_eq /mb_mapsto_def.
-        iFrame.
-      }
-      
-      iSplit. iPureIntro. set_solver +.
-      iSplit. iPureIntro. set_solver +.
-
-      iSplitL "excl5 own5".
-      {
-        rewrite excl_mapsto_eq /excl_mapsto_def.
-        rewrite own_mapsto_eq /own_mapsto_def.
-        iFrame.
-      }
-
-      iSplit; first done.
-      iSplit; first done.
-      
-      iExists mem5. unfold memory_pages. iSplit.
-      iPureIntro.
-      rewrite /retrieved_lending_memory_pages.
-      rewrite map_filter_empty pages_in_trans_empty union_empty_r_L //.
-      rewrite mem_mapsto_eq /mem_mapsto_def.
-      iFrame "Hmem2".
+      iApply "H".
     }
+    iApply "WP".
+    iApply (mtms_ftlr2 p_prog2 p_tx2 p_rx2 with "[-] []").
+    2: { iPureIntro. cbn. done. }
+    rewrite /mtms_interp_access2 /interp_access.
+    repeat (iSplit;[iPureIntro|]).
+    {
+      rewrite /mtms_slice_trans.
+      intros ? ? ? [|]; done.
+    }
+    {
+      rewrite /mtms_slice_rxs.
+      intros ?.
+      destruct os;done.
+    }
+    {
+      rewrite /mtms_slice_rxs.
+      intros ?.
+      destruct os;done.
+    }
+    {
+      rewrite /mtms_slice_rxs.
+      intros ??.
+      destruct os.
+      destruct p.
+      intros.
+      done.
+      done.
+    }
+    {
+      intros.
+      rewrite /mtms_slice_rxs //.
+    }
+
+    iSplitL "Hreg2".
+    iExists (get_reg_files σ !!! V2).
+    unfold get_reg_gmap_vm.
+    iSplit.
+    iPureIntro.
+    unfold base_extra.is_total_gmap.
+    apply Htotal_reg.
+    simpl.
+    {
+      set g := (λ p0 : reg_name * Addr, (p0.1, 2%fin, p0.2)).
+      unfold V2.
+      simpl.
+      set l := (σ.1.1.1.1.1 !!! 2%fin).
+      iEval (rewrite big_opM_map_to_list) in "Hreg2".
+      rewrite map_to_list_to_map.
+      rewrite big_opL_fmap.
+      subst g.
+      simpl.
+      rewrite big_opM_map_to_list.
+      iFrame "Hreg2".
+      subst g.
+      apply NoDup_fmap_fst.
+      intros [x1 x2] y1 y2 Hh Hh'.
+      rewrite elem_of_list_In in Hh.
+      rewrite elem_of_list_In in Hh'.
+      rewrite in_map_iff in Hh.
+      rewrite in_map_iff in Hh'.
+      destruct Hh as [(x & x') [Hheq Hh]].
+      destruct Hh' as [(t & t') [Hh'eq Hh']].
+      simpl in Hheq.
+      simpl in Hh'eq.
+      inversion Hheq.
+      inversion Hh'eq.
+      simplify_eq.
+      clear Hheq Hh'eq.
+      rewrite <-elem_of_list_In in Hh.
+      rewrite <-elem_of_list_In in Hh'.
+      apply map_to_list_unique with l x1; auto.
+      apply NoDup_fmap_2.
+      intros a b abeq.
+      inversion abeq.
+      destruct a, b; simpl in *.
+      by simplify_eq.
+      apply NoDup_map_to_list.
+    }
+    iFrame "VMProp2_half".
+    rewrite difference_empty_L.
+    unfold transaction_pagetable_entries_owned.
+    unfold retrieved_transaction_owned.
+    rewrite -!big_sepFM_empty.
+    assert (({[p_prog2; p_tx2; p_rx2]} ∖ {[p_rx2; p_tx2]}) = {[p_prog2]}) as ->.
+    {
+      rewrite !difference_union_distr_l_L.        
+      rewrite difference_disjoint_L.
+      assert ({[p_tx2]} ∖ {[p_rx2; p_tx2]} = ∅) as ->.
+      { set_solver +. }
+      assert ({[p_rx2]} ∖ {[p_rx2; p_tx2]} = ∅) as ->.
+      { set_solver +. }
+      set_solver +.
+      apply disjoint_singleton_l.
+      intros contra.
+      rewrite elem_of_union in contra.
+      rewrite !elem_of_singleton in contra.
+      solve_NoDup_pre'.
+      solve_NoDup_pre'' 2 9.
+      solve_NoDup_pre'' 2 6.
+    }
+    unfold pagetable_entries_excl_owned.
+    unfold logrel.pgt.
+    rewrite !big_sepS_singleton.
+    unfold tx_page.
+    iSplitL "mb2TX p_tx2 excl4 own4".
+    iSplitR "p_tx2".
+    rewrite mb_mapsto_eq /mb_mapsto_def.
+    rewrite excl_mapsto_eq own_mapsto_eq /excl_mapsto_def /own_mapsto_def.
+    iFrame.
+    iExists mem_p_tx2. unfold memory_page. iSplit. iPureIntro.
+    rewrite Hdom_mem_p_tx2.
+    apply set_of_addr_singleton.
+    rewrite mem_mapsto_eq /mem_mapsto_def.
+    iFrame "p_tx2".
+    rewrite access_mapsto_eq /access_mapsto_def /=.
+    assert ({[p_tx2; p_rx2; p_prog2]} = {[p_prog2; p_tx2; p_rx2]}) as -> by set_solver +.
+    iFrame "access3".
+    unfold rx_page.
+
+    iSplitL "mb2RX' excl3 own3".
+    {
+      rewrite excl_mapsto_eq /excl_mapsto_def.
+      rewrite own_mapsto_eq /own_mapsto_def.
+      rewrite mb_mapsto_eq /mb_mapsto_def.
+      iFrame.
+    }
+    
+    iSplit. iPureIntro. set_solver +.
+    iSplit. iPureIntro. set_solver +.
+
+    iSplitL "excl5 own5".
+    {
+      rewrite excl_mapsto_eq /excl_mapsto_def.
+      rewrite own_mapsto_eq /own_mapsto_def.
+      iFrame.
+    }
+
+    iSplit; first done.
+    iSplit; first done.
+    
+    iExists mem5. unfold memory_pages. iSplit.
+    iPureIntro.
+    rewrite /retrieved_lending_memory_pages.
+    rewrite map_filter_empty pages_in_trans_empty union_empty_r_L //.
+    rewrite mem_mapsto_eq /mem_mapsto_def.
+    iFrame "Hmem2".
    Qed.
 
 End mtms_adequacy.
