theories/examples/mem_trans_msg_send/proof.v
@@ -3,7 +3,7 @@ From HypVeri.algebra Require Import base base_extra mem pagetable trans.
 From HypVeri.rules Require Import rules_base mov halt run yield mem_send mem_retrieve
   mem_relinquish mem_reclaim ldr str msg_send msg_wait msg_poll add.
 From HypVeri.examples Require Import instr utils.
-From HypVeri.logrel Require Import logrel logrel_extra.
+From HypVeri.logrel Require Import logrel logrel_extra logrel_prim_extra fundamental.
 From HypVeri Require Import proofmode machine_extra.
 Require Import Setoid.
 
@@ -241,15 +241,6 @@ Section proof.
     let RX1 := (RX_state@V1 := None ∗ RX@V1:=prx1 ∗ ∃ mem_rx, memory_page prx1 mem_rx)%I in
     let RX2 := (RX_state@V2 := None ∗ RX@V2:=prx2 ∗ ∃ mem_rx, memory_page prx2 mem_rx)%I in
     let program0 := mtms_program0 in
-    (* of_pid pshare = addr -> *)
-    (* (* Disjoint pages *) *)
-    (* (of_pid ptx0 = i_ptx0) -> *)
-    (* (of_pid prx1 = i_prx1) -> *)
-    (* (pprog0 ∉ ({[pshare; ptx0; pprog2; ptx2; prx2]}:gset _)) -> *)
-    (* pshare ≠ prx0 -> *)
-    (* pshare ≠ pprog0 -> *)
-    (* pshare ≠ ptx0 -> *)
-    (* ptx0 ≠ prx0 -> *)
     (* Addresses-values connection *)
     seq_in_page (of_pid pprog0) (length program0) pprog0 ->
     (* Mem for program *)
@@ -295,7 +286,6 @@ Section proof.
                  )}}%I.
   Proof.
     rewrite /vmprop_unknown.
-(* Haddr Htxeq Hrxeq HnIn_p HneAddr_RX0 HneAddr_PG0 HneAddr_TX0 HneTX0_RX0  *)
     iIntros (HIn) "((p_1 & p_2 & p_3 & p_4 & p_5 & p_6 & p_7
             & p_8 & p_9 & p_10 & p_11 & p_12 & p_13 & p_14 & p_15 & p_16 
             & p_17 & p_18 & p_19 & p_20 & p_21 & p_22 & p_23 & p_24 & p_25
@@ -1004,32 +994,25 @@ Section proof.
       rewrite Heq_ptx0.
       split; reflexivity.
     }
-    (* TODO *)
-    iDestruct "txmem" as "(txmem1 & txacc)".    
+    iDestruct "txmem" as "(txmem1 & txacc)".
     iApply ((@str _ _ _ _ _ _ _ wh (encode_vmid V0) 1%Qp prx0 ptx0 {[pshare;pprog0; ptx0]} (pprog0 ^+ 23%nat)%f i_ptx0 R2 R5) with "[p_24 PCz acc txmem1 RX0page tx R2z R5z]").
     apply decode_encode_instruction.
-    apply union_subseteq_r'.
-    apply union_least.
-    rewrite singleton_subseteq_l.    
-    apply elem_of_union_r.
-    apply elem_of_singleton_2.
-    {
-      rewrite <-Heq_ptx0.
-      rewrite to_pid_aligned_eq.
-      reflexivity.
-    }
-    rewrite singleton_subseteq_l.
-    apply elem_of_union_l.
-    apply elem_of_singleton_2.
-    apply HIn.
-    apply finz_succN_in_seq; simpl; lia.
-    rewrite HIn.
+    rewrite <-Heq_ptx0.
     rewrite to_pid_aligned_eq.
-    assumption.
+    rewrite HIn.
+    set_solver +.
+    apply finz_succN_in_seq; simpl; lia.
+    rewrite HIn. done.
     apply finz_succN_in_seq; simpl; lia.
     rewrite <-Heq_ptx0.
     rewrite to_pid_aligned_eq.
-    assumption.
+    {
+      intros Heq.
+      feed pose proof (NoDup_lookup _ 4 7 prx0 Hps_nd).
+      rewrite Heq. done.
+      rewrite Heq. done.
+      lia.
+    }
     iFrame.
     iModIntro.
     iIntros "(PCz & _ & R5z & txmem1 & R2z & acc & tx & RX0page) _".
@@ -1041,14 +1024,10 @@ Section proof.
     iDestruct ("txacc" with "[$txmem1]") as "txmem".
     iApply ((@mov_reg _ _ _ _ _ _ _ wh 1%Qp {[pshare;pprog0; ptx0]} ptx0 (pprog0 ^+ 24%nat)%f one R3 R2) with "[PCz p_25 acc tx R2z R3z]").
     apply decode_encode_instruction.
-    apply elem_of_union_r.
-    apply elem_of_union_l.
-    apply elem_of_singleton_2.
-    apply HIn.
-    apply finz_succN_in_seq; simpl; lia.
     rewrite HIn.
-    rewrite to_pid_aligned_eq.
-    assumption.
+    set_solver +.
+    apply finz_succN_in_seq; simpl; lia.
+    rewrite HIn. done.
     apply finz_succN_in_seq; simpl; lia.
     iFrame.
     iModIntro.
@@ -1059,15 +1038,10 @@ Section proof.
     iEval (simpl) in "PCz".
     iApply ((@mov_word _ _ _ _ _ _ _ _ _ {[pshare;pprog0; ptx0]} ptx0 (pprog0 ^+ 25%nat)%f msg_send_I R0) with "[p_26 PCz acc tx R0z]").
     apply decode_encode_instruction.
-    apply elem_of_union_r.
-    apply elem_of_union_l.
-    apply elem_of_singleton_2.
     rewrite HIn.
-    reflexivity.
+    set_solver +.
     apply finz_succN_in_seq; simpl; lia.
-    rewrite HIn.
-    rewrite to_pid_aligned_eq.
-    assumption.
+    rewrite HIn. done.
     apply finz_succN_in_seq; simpl; lia.
     iFrame.
     iModIntro.
@@ -1078,15 +1052,10 @@ Section proof.
     iEval (simpl) in "PCz".
     iApply ((@mov_word _ _ _ _ _ _ _ _ _ {[pshare;pprog0; ptx0]} ptx0 (pprog0 ^+ 26%nat)%f (encode_vmid V1) R1) with "[p_27 PCz acc tx R1z]").
     apply decode_encode_instruction.
-    apply elem_of_union_r.
-    apply elem_of_union_l.
-    apply elem_of_singleton_2.
     rewrite HIn.
-    reflexivity.
+    set_solver +.
     apply finz_succN_in_seq; simpl; lia.
-    rewrite HIn.
-    rewrite to_pid_aligned_eq.
-    assumption.
+    rewrite HIn. done.
     apply finz_succN_in_seq; simpl; lia.
     iFrame.
     iModIntro.
@@ -1097,15 +1066,10 @@ Section proof.
     iEval (simpl) in "PCz".
     iApply ((@mov_word _ _ _ _ _ _ _ _ _ {[pshare;pprog0; ptx0]} ptx0 (pprog0 ^+ 27%nat)%f one R2) with "[p_28 PCz acc tx R2z]").
     apply decode_encode_instruction.
-    apply elem_of_union_r.
-    apply elem_of_union_l.
-    apply elem_of_singleton_2.
     rewrite HIn.
-    reflexivity.
+    set_solver +.
     apply finz_succN_in_seq; simpl; lia.
-    rewrite HIn.
-    rewrite to_pid_aligned_eq.
-    assumption.
+    rewrite HIn. done.
     apply finz_succN_in_seq; simpl; lia.
     iFrame.
     iModIntro.
@@ -1119,15 +1083,10 @@ Section proof.
     | |- context [([∗ map] k↦y ∈ ?p, k ->a y)%I] => set q' := p
     end.
     iApply ((@msg_send_primary _ _ _ _ _ hvc_I msg_send_I (encode_vmid V1) {[pshare;pprog0; ptx0]} ptx0 q' 1%Qp prx1 rxmem one (pprog0 ^+ 28%nat)%f V1) with "[p_29 PCz acc tx R0z R1z R2z txmem RX1st rxmem RX1page]").
-    rewrite HIn.
-    rewrite to_pid_aligned_eq.
-    assumption.
+    rewrite HIn. done.
     apply finz_succN_in_seq; simpl; lia.
-    apply elem_of_union_r.
-    apply elem_of_union_l.
-    apply elem_of_singleton_2.
     rewrite HIn.
-    reflexivity.
+    set_solver +.
     apply finz_succN_in_seq; simpl; lia.
     by rewrite decode_encode_instruction.
     by rewrite decode_encode_hvc_func.
@@ -1136,15 +1095,14 @@ Section proof.
     done.
     iFrame.
     iNext.
-    iPureIntro.
-    subst q'.
-    subst q.
+    iPureIntro. subst q'. subst q.
     rewrite dom_insert_L.
     rewrite subseteq_union_1_L.
     assumption.
     apply singleton_subseteq_l.
     apply elem_of_dom.
     exists (encode_vmid V0).
+    rewrite -Heq_ptx0.
     apply lookup_insert.
     iModIntro.
     iIntros "(PCz & _ & acc & R0z & R1z & R2z & tx & RX1page & RX1st & txmem & %descr & %descrlen & %descrsubseteq & rxmem) _".
@@ -1154,15 +1112,10 @@ Section proof.
     iEval (simpl) in "PCz".
     iApply ((@mov_word _ _ _ _ _ _ _ _ _ {[pshare;pprog0; ptx0]} ptx0 (pprog0 ^+ 29%nat)%f run_I R0) with "[p_30 PCz acc tx R0z]").
     apply decode_encode_instruction.
-    apply elem_of_union_r.
-    apply elem_of_union_l.
-    apply elem_of_singleton_2.
     rewrite HIn.
-    reflexivity.
+    set_solver +.
     apply finz_succN_in_seq; simpl; lia.
-    rewrite HIn.
-    rewrite to_pid_aligned_eq.
-    assumption.
+    rewrite HIn. done.
     apply finz_succN_in_seq; simpl; lia.
     iFrame.
     iModIntro.
@@ -1173,15 +1126,10 @@ Section proof.
     iEval (simpl) in "PCz".
     iApply ((@mov_word _ _ _ _ _ _ _ _ _ {[pshare;pprog0; ptx0]} ptx0 (pprog0 ^+ 30%nat)%f (encode_vmid V1) R1) with "[p_31 PCz acc tx R1z]").
     apply decode_encode_instruction.
-    apply elem_of_union_r.
-    apply elem_of_union_l.
-    apply elem_of_singleton_2.
     rewrite HIn.
-    reflexivity.
+    set_solver +.
     apply finz_succN_in_seq; simpl; lia.
-    rewrite HIn.
-    rewrite to_pid_aligned_eq.
-    assumption.
+    rewrite HIn. done.
     apply finz_succN_in_seq; simpl; lia.
     iFrame.
     iModIntro.
@@ -1221,28 +1169,22 @@ Section proof.
           apply elem_of_list_to_map_1.
           apply NoDup_singleton.
           rewrite <-Heq_ptx0.
-          rewrite to_pid_aligned_eq.
           apply elem_of_list_singleton.
           reflexivity.
         }
         apply lookup_insert_rev in descrsubseteq.
         by symmetry.
       }
-      rewrite Hrxeq.
+      rewrite Heq_prx1.
       apply lookup_insert.
     }    
     iApply ((@run _ _ _ _ _ hvc_I run_I (encode_vmid V1) 1%Qp {[pshare;pprog0; ptx0]} ptx0 ((PC @@ V0 ->r (pprog0 ^+ 32%nat)%f) ∗ (V0 -@A> {[pshare;pprog0; ptx0]}) ∗ (TX@V0:=ptx0))%I (R0 @@ V0 ->r run_I ∗ R1 @@ V0 ->r encode_vmid V1 ∗ addr ->a two  ∗ (∃ (wh : Addr), (∃ (β : mem), wh ->t (V0, V1, {[pshare]}, Sharing) ∗ wh ->re false ∗ (rx_state_mapsto V1 1 (Some (of_imm one, V0)) ∗ ⌜V0 ≠ V1⌝) ∗ RX@V1:=prx1 ∗ memory_page prx1 β ∗ ⌜β !! (of_imm i_prx1) = Some wh⌝) ∗
               VMProp V0 ((R0 @@ V0 ->r yield_I ∗ R1 @@ V0 ->r encode_vmid V1 ∗ addr ->a four ∗ wh ->t (V0, V1, {[pshare]}, Sharing) ∗ RX@V1:=prx1 ∗ (rx_state_mapsto V1 1 None ∗ True) ∗ (∃ mem_rx, memory_page prx1 mem_rx)) ∗
               VMProp V1 False%I (1/2)%Qp) (1/2)%Qp))%I True%I (pprog0 ^+ 31%nat)%f V1 True%I ((R0 @@ V0 ->r yield_I ∗ R1 @@ V0 ->r encode_vmid V1 ∗ addr ->a four ∗ wh ->t (V0, V1, {[pshare]}, Sharing) ∗ RX@V1:=prx1 ∗ (rx_state_mapsto V1 1 None ∗ True) ∗ (∃ mem_rx, memory_page prx1 mem_rx)) ∗ VMProp 1 False (1 / 2))%I) with "[PCz p_32 acc tx R0z R1z prop0 prop1 mem rxmem whretri whtans RX1page RX1st]").
-    apply elem_of_union_r.
-    apply elem_of_union_l.
-    apply elem_of_singleton_2.
     rewrite HIn.
-    reflexivity.
+    set_solver +.
     apply finz_succN_in_seq; simpl; lia.
-    rewrite HIn.
-    rewrite to_pid_aligned_eq.
-    assumption.
+    rewrite HIn. done.
     apply finz_succN_in_seq; simpl; lia.
     done.
     apply decode_encode_instruction.
@@ -1251,8 +1193,7 @@ Section proof.
     iSplitL "PCz p_32 acc tx R0z R1z".
     iFrame.
     iSplitL "prop1".
-    iNext.
-    simpl.
+    iNext. simpl.
     iExact "prop1".
     iFrame "prop0".
     iSplit; last done.
@@ -1266,9 +1207,7 @@ Section proof.
       iFrame.
       iExists wh.
       iSplitR "prop0".
-      iExists β.
-      simpl.
-      iFrame.
+      iExists β. simpl. iFrame.
       done.
       simpl.
       iFrame.
@@ -1283,15 +1222,10 @@ Section proof.
     rewrite wp_sswp.
     iApply ((@mov_word _ _ _ _ _ _ _ _ _ {[pshare;pprog0; ptx0]} ptx0 (pprog0 ^+ 32%nat)%f run_I R0) with "[p_33 PCz acc tx R0z]").
     apply decode_encode_instruction.
-    apply elem_of_union_r.
-    apply elem_of_union_l.
-    apply elem_of_singleton_2.
     rewrite HIn.
-    reflexivity.
+    set_solver +.
     apply finz_succN_in_seq; simpl; lia.
-    rewrite HIn.
-    rewrite to_pid_aligned_eq.
-    assumption.
+    rewrite HIn. done.
     apply finz_succN_in_seq; simpl; lia.
     iFrame.
     iModIntro.
@@ -1302,15 +1236,10 @@ Section proof.
     iEval (simpl) in "PCz".
     iApply ((@mov_word _ _ _ _ _ _ _ _ _ {[pshare;pprog0; ptx0]} ptx0 (pprog0 ^+ 33%nat)%f (encode_vmid V2) R1) with "[p_34 PCz acc tx R1z]").
     apply decode_encode_instruction.
-    apply elem_of_union_r.
-    apply elem_of_union_l.
-    apply elem_of_singleton_2.
     rewrite HIn.
-    reflexivity.
+    set_solver +.
     apply finz_succN_in_seq; simpl; lia.
-    rewrite HIn.
-    rewrite to_pid_aligned_eq.
-    assumption.
+    rewrite HIn. done.
     apply finz_succN_in_seq; simpl; lia.
     iFrame.
     iModIntro.
@@ -1319,16 +1248,13 @@ Section proof.
     iEval (rewrite finz_plus_one_simpl) in "PCz".
     rewrite Z_of_nat_simpl.
     iEval (simpl) in "PCz".    
-    iApply ((@run _ _ _ _ _ hvc_I run_I (encode_vmid V2) 1%Qp {[pshare;pprog0; ptx0]} ptx0 ((PC @@ V0 ->r (pprog0 ^+ 35%nat)%f) ∗ (V0 -@A> {[pshare;pprog0; ptx0]}) ∗ (TX@V0:=ptx0))%I (fixpoint (vmprop_unknown_pre V2) ∅) ((R0 @@ V0 ->r yield_I ∗ R1 @@ V0 ->r encode_vmid V1 ∗ addr ->a finz.FinZ 4 four_obligation_1 four_obligation_2 ∗ wh ->t (V0, V1, {[pshare]}, Sharing) ∗ RX@V1:=prx1 ∗ (rx_state_mapsto V1 1 None ∗ True) ∗ (∃ mem_rx : mem, memory_page prx1 mem_rx)) ∗ VMProp 1 False (1 / 2))%I (pprog0 ^+ 34%nat)%f V2 (trans.fresh_handles 1 (valid_handles ∖ {[wh]}) ∗ (∃ mem_rx : mem, memory_page prx0 mem_rx) ∗ (∃ mem_rx : mem, memory_page prx1 mem_rx) ∗ (∃ mem_rx : mem, memory_page prx2 mem_rx) ∗ RX@V0:=prx0 ∗ RX@V1:=prx1 ∗ RX@V2:=prx2 ∗ rx_state_mapsto V0 1 None ∗ (rx_state_mapsto V1 1 None ∗ True) ∗ rx_state_mapsto V2 1 None ∗ ([∗ set] p ∈ {[pshare]}, p -@O> V0 ∗ p -@E> false) ∗ R2 @@ V0 ->r one)%I (vmprop_zero V2 (<[wh := ((V0, V1, ({[pshare]} : gset PID), Sharing), true)]> ∅) (<[V2 := None]>(<[V1 := None]>(<[V0 := None]>∅))))%I) with "[PCz p_35 acc tx R0z R1z prop0 prop2 whfresh RX0page RX0mem RX0st RX1page RX1mem RX1st RX2page RX2mem RX2st R2z OE whtrans]").
-    apply elem_of_union_r.
-    apply elem_of_union_l.
-    apply elem_of_singleton_2.
+    iApply ((@run _ _ _ _ _ hvc_I run_I (encode_vmid V2) 1%Qp {[pshare;pprog0; ptx0]} ptx0 ((PC @@ V0 ->r (pprog0 ^+ 35%nat)%f) ∗ (V0 -@A> {[pshare;pprog0; ptx0]}) ∗ (TX@V0:=ptx0))%I
+               (vmprop_unknown V2 mtms_slice_trans mtms_slice_rxs ∅) ((R0 @@ V0 ->r yield_I ∗ R1 @@ V0 ->r encode_vmid V1 ∗ addr ->a finz.FinZ 4 four_obligation_1 four_obligation_2 ∗ wh ->t (V0, V1, {[pshare]}, Sharing) ∗ RX@V1:=prx1 ∗ (rx_state_mapsto V1 1 None ∗ True) ∗ (∃ mem_rx : mem, memory_page prx1 mem_rx)) ∗ VMProp 1 False (1 / 2))%I (pprog0 ^+ 34%nat)%f V2 (trans.fresh_handles 1 (valid_handles ∖ {[wh]}) ∗ (∃ mem_rx : mem, memory_page prx0 mem_rx) ∗ (∃ mem_rx : mem, memory_page prx1 mem_rx) ∗ (∃ mem_rx : mem, memory_page prx2 mem_rx) ∗ RX@V0:=prx0 ∗ RX@V1:=prx1 ∗ RX@V2:=prx2 ∗ rx_state_mapsto V0 1 None ∗ (rx_state_mapsto V1 1 None ∗ True) ∗ rx_state_mapsto V2 1 None ∗ ([∗ set] p ∈ {[pshare]}, p -@O> V0 ∗ p -@E> false) ∗ R2 @@ V0 ->r one)%I
+               (vmprop_zero V2 mtms_slice_trans mtms_slice_rxs (<[wh := ((V0, V1, ({[pshare]} : gset PID), Sharing), true)]> ∅) (<[V2 := None]>(<[V1 := None]>(<[V0 := None]>∅))))%I) with "[PCz p_35 acc tx R0z R1z prop0 prop2 whfresh RX0page RX0mem RX0st RX1page RX1mem RX1st RX2page RX2mem RX2st R2z OE whtrans]").
     rewrite HIn.
-    reflexivity.
+    set_solver +.
     apply finz_succN_in_seq; simpl; lia.
-    rewrite HIn.
-    rewrite to_pid_aligned_eq.
-    assumption.
+    rewrite HIn. done.
     apply finz_succN_in_seq; simpl; lia.
     done.
     apply decode_encode_instruction.
@@ -1343,160 +1269,164 @@ Section proof.
       iEval (simpl) in "PCz".    
       iFrame.
       iApply vmprop_unknown_eq.
-      iExists (<[wh := ((V0, V1, ({[pshare]} : gset PID), Sharing), true)]> ∅), (<[V2 := None]>(<[V1 := None]>(<[V0 := None]>∅))).
+      iExists ({[wh := ((V0, V1, ({[pshare]} : gset PID), Sharing), true)]}), (<[V2 := None]>(<[V1 := None]>(<[V0 := None]>∅))).
       iSplit.
-      - iPureIntro.
-        unfold trans_rel_secondary.
-        split.
-        rewrite insert_empty.
-        rewrite map_filter_singleton_False.
-        rewrite map_filter_empty.
-        rewrite fmap_empty.
-        reflexivity.
+      iPureIntro.
+      unfold trans_rel_secondary.
+      split.
+      rewrite map_filter_singleton_False.
+      rewrite map_filter_empty.
+      rewrite fmap_empty //.
+      simpl.
+      intros [? _]. done.
+      rewrite map_filter_singleton_False.
+      rewrite map_filter_empty //.
+      intros [? _]. done.
+      iSplitL "whfresh OE whtrans".
+      unfold transaction_hpool_global_transferred.
+      iExists (valid_handles ∖ {[wh]}). simpl.
+      rewrite wheq.
+      rewrite difference_diag_L.
+      rewrite union_empty_l_L.
+      iSplit.
+      rewrite dom_singleton_L //.
+      rewrite big_opM_singleton.
+      rewrite elem_of_singleton.
+      simpl.
+      rewrite bool_decide_eq_false_2.
+      unfold pgt_3_4. unfold pgt.
+      rewrite !big_opS_singleton.
+      unfold valid_transaction.
+      simpl.
+      iFrame.
+      iSplitL "whtrans".
+      iDestruct "whtrans" as "(whtrans & %P1 & %P2)".
+      iSplit.
+      rewrite trans_mapsto_eq /trans_mapsto_def.            
+      iDestruct (ghost_map_elem_split with "whtrans") as "[H1 H2]".
+      iFrame.
+      iPureIntro.
+      split; done.            
+      iDestruct "OE" as "(O & E)".
+      iDestruct (own_split with "O") as "(O1 & O2)".
+      iDestruct (own_split with "O2") as "(O2 & O3)".
+      iDestruct (excl_split with "E") as "(E1 & E2)".
+      iDestruct (excl_split with "E2") as "(E2 & E3)".
+      rewrite half_of_half.
+      iFrame.
+      intros contra; contradiction.
+      iSplitR.
+      rewrite transferred_only_equiv.
+      unfold transaction_pagetable_entries_transferred.
+      rewrite big_sepFM_insert_False.
+      iSplitR. iApply big_sepFM_empty.
+      2: {
         intros contra.
-        simpl in contra.
-        destruct contra.
-        discriminate.
-        rewrite map_filter_singleton_False.
-        rewrite map_filter_empty.
+        destruct contra; discriminate.
+      }
+      2: apply lookup_empty.
+      iSplitR.
+      unfold retrievable_transaction_transferred.
+      iSplitL.
+      rewrite big_sepFM_insert_False.
+      iApply big_sepFM_empty.
+      intros contra.
+      destruct contra; discriminate.
+      apply lookup_empty.
+      rewrite big_sepFM_insert_False.
+      iApply big_sepFM_empty.
+      intros contra.
+      destruct contra; discriminate.
+      apply lookup_empty.
+      iExists ∅.
+      unfold memory_pages.
+      iSplit; last done.
+      iPureIntro.
+      unfold transferred_memory_pages.
+      rewrite dom_empty_L.
+      rewrite map_filter_singleton_False.
+      rewrite pages_in_trans_empty.
+      rewrite set_of_addr_empty //.
+      intros contra.
+      destruct contra as [contra ?].
+      destruct contra; discriminate.
+      {
+        intros. rewrite /mtms_slice_trans //.
+      }
+      {
+        rewrite /trans_neq.
+        rewrite map_Forall_singleton.
+        simpl. done.
+      }
+      {
+        rewrite /trans_ps_disj.
+        rewrite /inv_trans_ps_disj'.
+        rewrite /lift_option_gmap.
+        rewrite map_fmap_singleton.
+        rewrite map_Forall_singleton.
+        rewrite delete_singleton.
+        rewrite /pages_in_trans'.
+        rewrite map_fold_empty.
+        set_solver +.
+      }
+      iSplitL "R0z".
+      iExists run_I.
+      iFrame.
+      iPureIntro.
+      apply decode_encode_hvc_func.
+      iSplitL "R1z".
+      iExists (encode_vmid V2).
+      iFrame.
+      iPureIntro.
+      apply decode_encode_vmid.
+      iSplitL "R2z".
+      iExists one.
+      iFrame.
+      iSplitL "RX2mem RX2page RX2st".
+      iIntros.
+      rewrite lookup_insert in H.
+      inversion H. subst rs.
+      unfold rx_state_match.
+      iFrame.
+      iExists prx2.
+      iFrame.
+      iSplitR "prop0".
+      unfold rx_states_global.
+      rewrite delete_insert.
+      unfold rx_state_match.
+      rewrite insert_empty.
+      rewrite big_opM_insert_delete.
+      iFrame "RX1st".
+      iSplitL "RX1page RX1mem".
+      iExists prx1.
+      iFrame.
+      assert (delete V1 {[V0 := None]} = {[V0 := None]}) as ->.
+      {
+        rewrite delete_notin.
         reflexivity.
-        intros contra.
-        simpl in contra.
-        destruct contra.
-        discriminate.
-      - iSplitL "whfresh OE whtrans".
-        + unfold transaction_hpool_global_transferred.
-          iExists (valid_handles ∖ {[wh]}).
-          simpl.
-          iSplit.
-          rewrite wheq.
-          rewrite difference_diag_L.
-          rewrite insert_empty.
-          rewrite union_empty_l_L.
-          iPureIntro.
-          set_solver +.
-          rewrite wheq.
-          rewrite difference_diag_L.
-          rewrite insert_empty.
-          rewrite big_opM_singleton.
-          rewrite elem_of_singleton.
-          simpl.
-          rewrite bool_decide_eq_false_2.
-          unfold pgt_3_4.
-          unfold pgt.
-          rewrite !big_opS_singleton.
-          unfold valid_transaction.
-          simpl.
-          iFrame.
-          iSplitL "whtrans".
-          * iDestruct "whtrans" as "(whtrans & %P1 & %P2)".
-            iSplit.
-            rewrite trans_mapsto_eq /trans_mapsto_def.            
-            iDestruct (ghost_map_elem_split with "whtrans") as "[H1 H2]".
-            iFrame.
-            iPureIntro.
-            split; done.            
-          * iDestruct "OE" as "(O & E)".            
-            iDestruct (own_split with "O") as "(O1 & O2)".
-            iDestruct (own_split with "O2") as "(O2 & O3)".
-            iDestruct (excl_split with "E") as "(E1 & E2)".
-            iDestruct (excl_split with "E2") as "(E2 & E3)".
-            rewrite half_of_half.
-            iFrame.
-          * intros contra; contradiction.
-        + iSplitR.
-          * unfold transaction_pagetable_entries_transferred.
-            rewrite big_sepFM_insert_False.
-            iApply big_sepFM_empty.
-            intros contra.
-            destruct contra; discriminate.
-            apply lookup_empty.
-          * iSplitR.
-            -- unfold retrievable_transaction_transferred.
-               iSplitL.
-               rewrite big_sepFM_insert_False.
-               iApply big_sepFM_empty.
-               intros contra.
-               destruct contra; discriminate.
-               apply lookup_empty.
-               rewrite big_sepFM_insert_False.
-               iApply big_sepFM_empty.
-               intros contra.
-               destruct contra; discriminate.
-               apply lookup_empty.
-            -- iSplitR.
-               ++ iExists ∅.
-                  unfold memory_pages.
-                  iSplit; last done.
-                  iPureIntro.
-                  unfold transferred_memory_pages.
-                  rewrite dom_empty_L.
-                  rewrite insert_empty.
-                  rewrite map_filter_singleton_False.
-                  rewrite pages_in_trans_empty.
-                  rewrite set_of_addr_empty.
-                  reflexivity.
-                  intros contra.
-                  destruct contra as [contra ?].
-                  destruct contra; discriminate.
-               ++ iSplitL "R0z".
-                  ** iExists run_I.
-                     iFrame.
-                     iPureIntro.
-                     apply decode_encode_hvc_func.
-                  ** iSplitL "R1z".
-                     --- iExists (encode_vmid V2).
-                         iFrame.
-                         iPureIntro.
-                         apply decode_encode_vmid.
-                     --- iSplitL "R2z".
-                         +++ iExists one.
-                             iFrame.
-                         +++ iSplitL "RX2mem RX2page RX2st".
-                             unfold rx_state_get.
-                             iSplitR "RX2mem RX2page".
-                             *** iIntros (rs) "%contra".
-                                 apply lookup_insert_rev in contra.
-                                 rewrite <-contra.
-                                 iFrame.
-                             *** iExists prx2.
-                                 iFrame.
-                             *** iSplitR "prop0".
-                                 ---- unfold rx_states_global.
-                                      rewrite delete_insert.
-                                      unfold rx_state_match.
-                                      rewrite insert_empty.
-                                      rewrite big_opM_insert_delete.
-                                      iFrame "RX1st".
-                                      iSplitL "RX1page RX1mem".
-                                      iExists prx1.
-                                      iFrame.
-                                      assert (delete V1 {[V0 := None]} = {[V0 := None]}) as ->.
-                                      {
-                                        rewrite delete_notin.
-                                        reflexivity.
-                                        apply lookup_singleton_ne.
-                                        done.
-                                      }
-                                      rewrite big_opM_singleton.
-                                      iSplitL "RX0st"; first iFrame.
-                                      iExists prx0.
-                                      iFrame.
-                                      rewrite insert_empty.
-                                      rewrite lookup_insert_None.
-                                      split; last done.
-                                      by apply lookup_singleton_ne.
-                                 ---- iSplit.
-                                      ++++ iPureIntro.
-                                           unfold base_extra.is_total_gmap.
-                                           intros k.
-                                           rewrite insert_empty.
-                                           pose proof (in_list_of_vmids k) as G.
-                                           unfold list_of_vmids in G.
-                                           rewrite /vm_count /rywu_vmconfig /= in G.
-                                           rewrite /V2 /V1 /V0 /=.
-                                           destruct G as [<- | [<- | [<- | ?]]]; last contradiction; done.
-                                      ++++ iFrame.
+        apply lookup_singleton_ne.
+        done.
+      }
+      rewrite big_opM_singleton.
+      iSplitL "RX0st"; first iFrame.
+      iExists prx0.
+      iFrame.
+      rewrite insert_empty.
+      rewrite lookup_insert_None.
+      split; last done.
+      by apply lookup_singleton_ne.
+      iSplit.
+      iPureIntro.
+      unfold base_extra.is_total_gmap.
+      intros k.
+      rewrite insert_empty.
+      pose proof (in_list_of_vmids k) as G.
+      unfold list_of_vmids in G.
+      rewrite /vm_count /mtms_vmconfig /= in G.
+      simpl.
+      rewrite /V2 /V1 /V0 /=.
+      destruct G as [<- | [<- | [<- | ?]]]; last contradiction; done.
+      iFrame.
     }
     iModIntro.
     iIntros "[(PCz & acc & tx) prop0] Hholds".
@@ -1507,15 +1437,10 @@ Section proof.
     rewrite wp_sswp.
     clear -HIn Hnottx.
     iApply ((halt (pprog0 ^+ 35%nat)%f) with "[PCz p_36 acc tx]"); iFrameAutoSolve.
-    apply elem_of_union_r.
-    apply elem_of_union_l.
-    apply elem_of_singleton_2.
     rewrite HIn.
-    reflexivity.
+    set_solver +.
     apply finz_succN_in_seq; simpl; lia.
-    rewrite HIn.
-    rewrite to_pid_aligned_eq.
-    assumption.
+    rewrite HIn. done.
     apply finz_succN_in_seq; simpl; lia.
     iNext.
     iIntros "(PCz & _ & acc & tx)".
@@ -1529,29 +1454,18 @@ Section proof.
     done.
   Qed.
 
-  Lemma mtms_machine1 p_pg1 (p_tx1 : PID) prx1 (addr : Imm) (i_prx1 : Imm) :
-    let program1 := mtms_program1 addr i_prx1 in
-    of_pid pshare = addr ->
-    (* Disjoint pages *)
-    (* (of_pid p_tx1 = p_tx1imm) -> *)
-    (of_pid prx1 = i_prx1) ->
-    (* (of_pid p_pg1 = p_pg1imm) -> *)
-    (p_pg1 ∉ ({[pshare; p_tx1; prx1]}:gset _)) ->
-    pshare ≠ prx1 ->
-    pshare ≠ p_pg1 ->
-    pshare ≠ p_tx1 ->
-    p_tx1 ≠ prx1 ->
+  Lemma mtms_machine1 :
     (* Addresses-values connection *)
-    seq_in_page (of_pid p_pg1) (length program1) p_pg1 ->
+    seq_in_page (of_pid pprog1) (length mtms_program1) pprog1 ->
     (* Mem for program *)
-    (program (program1) (of_pid p_pg1)) ∗
+    (program (mtms_program1) (of_pid pprog1)) ∗
     (* TX mem *)
-    (∃ txmem, memory_page (tpa p_tx1) txmem) ∗
-    V1 -@A> (union (union (singleton p_pg1) (singleton (tpa p_tx1))) (singleton (tpa prx1))) ∗
+    (∃ txmem, memory_page ptx1 txmem) ∗
+    V1 -@A> {[pprog1;ptx1;prx1]} ∗
     (* TX page *)            
-    TX@ V1 := (tpa p_tx1) ∗
+    TX@ V1 := ptx1 ∗
     (* Program counter *)                      
-    PC @@ V1 ->r (of_pid p_pg1) ∗
+    PC @@ V1 ->r (of_pid pprog1) ∗
     (* Work registers *)                        
     (∃ r0, R0 @@ V1 ->r r0) ∗
     (∃ r1, R1 @@ V1 ->r r1) ∗
@@ -1565,8 +1479,7 @@ Section proof.
         VMProp V1 False%I (1/2)%Qp) (1/2)%Qp))%I (1/2)%Qp
     ⊢ VMProp_holds V1 (1/2)%Qp -∗ WP ExecI @ V1 {{ (λ m, False) }}%I.
   Proof.
-    iIntros (program1 Haddr (* Heq_ptx0 *) Hrxeq (* Hpgeq *) HnIn_p HneAddr_RX1 HneAddr_PG1 HneAddr_TX1 HneTX1_RX1 HIn).
-    iIntros "((p_1 & p_2 & p_3 & p_4 & p_5 & p_6 & p_7 
+    iIntros (HIn) "((p_1 & p_2 & p_3 & p_4 & p_5 & p_6 & p_7
             & p_8 & p_9 & p_10 & p_11 & p_12 & p_13 & p_14 & _)
          & (%txmemgm & txmem) & acc & tx & PCs & (%r0 & R0s) & (%r1 & R1s) & (%r2 & R2s)
          & (%r3 & R3s) & (%r4 & R4s) & (%r5 & R5s) 
@@ -1578,15 +1491,21 @@ Section proof.
     fold_finz_plus_one.
     repeat (rewrite finz_succN_correct).
     clear HIn; rename Hforall into HIn.
-    assert (p_pg1 ≠ p_tx1) as Hnottx. set_solver + HnIn_p.
+    assert (pprog1 ≠ ptx1) as Hnottx.
+    {
+      intros Heq.
+      feed pose proof (NoDup_lookup _ 1 5 ptx1 Hps_nd).
+      rewrite Heq. done.
+      rewrite Heq. done.
+      lia.
+    }
     rewrite wp_sswp.
     iDestruct "P" as "(R0z & R1z & mem & temp)".
-    iApply ((mov_word (of_pid p_pg1) i_prx1 R5) with "[p_1 PCs acc tx R5s]"); iFrameAutoSolve.
-    do 2 apply elem_of_union_l.
-    apply elem_of_singleton_2.
-    by rewrite to_pid_aligned_eq.
-    rewrite !to_pid_aligned_eq.
-    assumption.
+    iApply ((mov_word (of_pid pprog1) i_prx1 R5) with "[p_1 PCs acc tx R5s]"); iFrameAutoSolve.
+    rewrite to_pid_aligned_eq.
+    set_solver +.
+    rewrite to_pid_aligned_eq.
+    done.
     iNext.
     iDestruct "temp" as "(%wh & (%rxmem & (whtrans & whretri & RX1st & RX1page & RX1mem & %Hrxmem)) & prop0)".
     iIntros "(PCs & _ & acc & tx & R5s) _".
@@ -1594,24 +1513,26 @@ Section proof.
     iEval (unfold memory_page) in "RX1mem".
     iDestruct "RX1mem" as "(%rxmemdom & RX1mem)".
     iDestruct (@mem_big_sepM_split_upd _ _ i_prx1 wh with "RX1mem") as "(rxbase & rxmemacc)"; auto.
-    iApply ((ldr (p := p_tx1) (w1 := ldr_I R4 R5) (s := {[p_pg1; tpa p_tx1; tpa prx1]}) (w2 := wh) (w3 := r4) (q := 1%Qp) (p_pg1 ^+ 1)%f i_prx1 R4 R5) with "[PCs p_2 acc tx R4s R5s rxbase]").
+    rewrite -Heq_prx1.
+    iApply ((ldr (p := ptx1) (w1 := ldr_I R4 R5) (s := {[pprog1; ptx1; prx1]}) (w2 := wh) (w3 := r4) (q := 1%Qp) (pprog1 ^+ 1)%f i_prx1 R4 R5) with "[PCs p_2 acc tx R4s R5s rxbase]").
     by rewrite decode_encode_instruction.
-    apply union_subseteq.
-    split; rewrite singleton_subseteq_l.
-    do 2 apply elem_of_union_l.
-    apply elem_of_singleton_2.    
-    rewrite HIn.
-    reflexivity.
-    set_solver +.
-    rewrite <-Hrxeq.
-    set_solver +.
-    rewrite <-Hrxeq.
+    rewrite -Heq_prx1.
     rewrite to_pid_aligned_eq.
-    intros contra; exfalso; apply HneTX1_RX1; symmetry; assumption.
     rewrite HIn.
-    assumption.
     set_solver +.
+    set_solver +.
+    rewrite -Heq_prx1.
     rewrite to_pid_aligned_eq.
+    {
+      intros Heq.
+      feed pose proof (NoDup_lookup _ 5 8 ptx1 Hps_nd).
+      rewrite Heq. done.
+      rewrite Heq. done.
+      lia.
+    }
+    rewrite HIn. done.
+    set_solver +.
+    rewrite -Heq_prx1.
     iFrame.
     iModIntro.
     iIntros "(PCs & _ & R5s & rxbase & R4s & acc & tx) _".
@@ -1620,15 +1541,12 @@ Section proof.
     iEval (repeat (rewrite finz_succN_idemp)) in "PCs".
     iEval (simpl) in "PCs".
     iEval (repeat (rewrite finz_succN_correct)) in "PCs".
-    iApply ((mov_word (w3 := r0) (p_tx := p_tx1) (w1 := mov_word_I R0 msg_poll_I) (q := 1%Qp) (s := {[p_pg1; tpa p_tx1; tpa prx1]}) (p_pg1 ^+ 2%nat)%f msg_poll_I R0) with "[p_3 PCs acc tx R0s]").
+    iApply ((mov_word (w3 := r0) (p_tx := ptx1) (w1 := mov_word_I R0 msg_poll_I) (q := 1%Qp) (s := {[pprog1; ptx1; prx1]}) (pprog1 ^+ 2%nat)%f msg_poll_I R0) with "[p_3 PCs acc tx R0s]").
     by rewrite decode_encode_instruction.
-    do 2 apply elem_of_union_l.
-    apply elem_of_singleton_2.    
     rewrite HIn.
-    reflexivity.
+    set_solver +.
     apply finz_succN_in_seq; simpl; lia.
-    rewrite HIn.
-    assumption.
+    rewrite HIn. done.
     apply finz_succN_in_seq; simpl; lia.
     iFrame.
     iModIntro.
@@ -1637,7 +1555,7 @@ Section proof.
     iEval (rewrite finz_plus_one_simpl) in "PCs".
     rewrite Z_of_nat_simpl.
     iEval (simpl) in "PCs".
-    iApply ((msg_poll_full (r0 := msg_poll_I) (r1 := r1) (r2 := r2) (wi := hvc_I) (l := one) (i := V1) (j := V0) (p_tx := p_tx1) (q := 1%Qp) (s := {[p_pg1; tpa p_tx1; tpa prx1]}) (p_pg1 ^+ 3%nat)%f) with "[p_4 PCs acc tx R0s R1s R2s RX1st]").
+    iApply ((msg_poll_full (r0 := msg_poll_I) (r1 := r1) (r2 := r2) (wi := hvc_I) (l := one) (i := V1) (j := V0) (p_tx := ptx1) (q := 1%Qp) (s := {[pprog1; ptx1; prx1]}) (pprog1 ^+ 3%nat)%f) with "[p_4 PCs acc tx R0s R1s R2s RX1st]").
     do 2 apply elem_of_union_l.
     apply elem_of_singleton_2.    
     rewrite HIn.
@@ -1655,17 +1573,14 @@ Section proof.
     iEval (rewrite finz_plus_one_simpl) in "PCs".
     rewrite Z_of_nat_simpl.
     iEval (simpl) in "PCs".
-    iApply ((@mov_reg _ _ _ _ _ _ _ wh 1%Qp {[p_pg1; tpa p_tx1; tpa prx1]} (tpa p_tx1) (p_pg1 ^+ 4%nat)%f one R1 R4) with "[PCs p_5 acc tx R1s R4s]").
+    iApply ((@mov_reg _ _ _ _ _ _ _ wh 1%Qp {[pprog1; ptx1; prx1]} ptx1 (pprog1 ^+ 4%nat)%f one R1 R4) with "[PCs p_5 acc tx R1s R4s]").
     apply decode_encode_instruction.
     do 2 apply elem_of_union_l.    
     apply elem_of_singleton_2.
     apply HIn.
     apply finz_succN_in_seq; simpl; lia.
-    rewrite HIn.
-    rewrite to_pid_aligned_eq.
-    assumption.
+    rewrite HIn. done.
     apply finz_succN_in_seq; simpl; lia.
-    rewrite to_pid_aligned_eq.
     iFrame.
     iModIntro.
     iIntros "(PCs & _ & acc & tx & R1s & R4s) _".
@@ -1673,16 +1588,12 @@ Section proof.
     iEval (rewrite finz_plus_one_simpl) in "PCs".
     rewrite Z_of_nat_simpl.
     iEval (simpl) in "PCs".
-    iApply ((@mov_word _ _ _ _ _ _ _ _ _ {[p_pg1; tpa p_tx1; tpa prx1]} (tpa p_tx1) (p_pg1 ^+ 5%nat)%f mem_retrieve_I R0) with "[p_6 PCs acc tx R0s]").
+    iApply ((@mov_word _ _ _ _ _ _ _ _ _ {[pprog1; ptx1; prx1]} ptx1 (pprog1 ^+ 5%nat)%f mem_retrieve_I R0) with "[p_6 PCs acc tx R0s]").
     apply decode_encode_instruction.
-    do 2 apply elem_of_union_l.
-    apply elem_of_singleton_2.
     rewrite HIn.
-    reflexivity.
+    set_solver +.
     apply finz_succN_in_seq; simpl; lia.
-    rewrite HIn.
-    rewrite to_pid_aligned_eq.
-    assumption.
+    rewrite HIn. done.
     apply finz_succN_in_seq; simpl; lia.
     iFrame.
     iModIntro.
@@ -1691,43 +1602,43 @@ Section proof.
     iEval (rewrite finz_plus_one_simpl) in "PCs".
     rewrite Z_of_nat_simpl.
     iEval (simpl) in "PCs".
+    rewrite -Heq_prx1.
     iSpecialize ("rxmemacc" $! wh with "rxbase").
-    iApply ((mem_retrieve_share (sacc := {[p_pg1; tpa p_tx1; tpa prx1]}) (p_tx := tpa p_tx1) (p_pg1 ^+ 6%nat)%f wh) with "[PCs p_7 R0s R1s acc tx whretri whtrans RX1page RX1st rxmemacc]").
-    rewrite to_pid_aligned_eq.
-    rewrite HIn.
-    assumption.
+    iApply ((mem_retrieve_share (sacc := {[pprog1; ptx1; prx1]}) (p_tx := ptx1) (pprog1 ^+ 6%nat)%f wh) with "[PCs p_7 R0s R1s acc tx whretri whtrans RX1page RX1st rxmemacc]").
+    rewrite HIn. done.
     apply finz_succN_in_seq; simpl; lia.
-    do 2 apply elem_of_union_l.
-    apply elem_of_singleton_2.
     rewrite HIn.
-    reflexivity.
+    set_solver +.
     apply finz_succN_in_seq; simpl; lia.
     apply decode_encode_instruction.
     apply decode_encode_hvc_func.
-    iFrame.
-    iNext.
+    iFrame "PCs p_7 R0s R1s acc tx RX1st".
+    iFrame "whretri". iSplitL "whtrans".
+    iExact "whtrans".
+    iSplitL "RX1page". iExact "RX1page".
+    rewrite /memory_page. iSplit.
+    2: { iExact "rxmemacc". }
     iPureIntro.
-    rewrite dom_insert_lookup_L.
-    assumption.
-    exists wh.
-    assumption.
-    iModIntro.
+    rewrite -rxmemdom.
+    rewrite !dom_insert_lookup_L;cbn. done.
+    rewrite -?elem_of_dom;
+      try rewrite !dom_insert_lookup_L -?elem_of_dom.
+    rewrite rxmemdom.
+    rewrite elem_of_list_to_set.
+    rewrite elem_of_addr_of_page_iff.
+    rewrite to_pid_aligned_eq //.
+    iNext.
     iIntros "(PCs & _ & R0s & R1s & acc & tx & whretri & whtrans & RX1page & (%l & %des & (RX1st & _) & %deslen & %desshape & RX1mem)) _".
     rewrite wp_sswp.
     iEval (rewrite finz_plus_one_simpl) in "PCs".
     rewrite Z_of_nat_simpl.
     iEval (simpl) in "PCs".
-    iApply ((@mov_word _ _ _ _ _ _ _ _ _ ({[pshare]} ∪ {[p_pg1; tpa p_tx1; tpa prx1]}) (tpa p_tx1) (p_pg1 ^+ 7%nat)%f four R3) with "[p_8 PCs acc tx R3s]").
+    iApply ((@mov_word _ _ _ _ _ _ _ _ _ ({[pshare]} ∪ {[pprog1; ptx1; prx1]}) ptx1 (pprog1 ^+ 7%nat)%f four R3) with "[p_8 PCs acc tx R3s]").
     apply decode_encode_instruction.
-    apply elem_of_union_r.
-    do 2 apply elem_of_union_l.
-    apply elem_of_singleton_2.
     rewrite HIn.
-    reflexivity.
+    set_solver +.
     apply finz_succN_in_seq; simpl; lia.
-    rewrite HIn.
-    rewrite to_pid_aligned_eq.
-    assumption.
+    rewrite HIn. done.
     apply finz_succN_in_seq; simpl; lia.
     iFrame.
     iModIntro.
@@ -1736,17 +1647,12 @@ Section proof.
     iEval (rewrite finz_plus_one_simpl) in "PCs".
     rewrite Z_of_nat_simpl.
     iEval (simpl) in "PCs".
-    iApply ((@mov_word _ _ _ _ _ _ _ _ _ ({[pshare]} ∪ {[p_pg1; tpa p_tx1; tpa prx1]}) (tpa p_tx1) (p_pg1 ^+ 8%nat)%f addr R5) with "[p_9 PCs acc tx R5s]").
+    iApply ((@mov_word _ _ _ _ _ _ _ _ _ ({[pshare]} ∪ {[pprog1; ptx1; prx1]}) ptx1 (pprog1 ^+ 8%nat)%f addr R5) with "[p_9 PCs acc tx R5s]").
     apply decode_encode_instruction.
-    apply elem_of_union_r.
-    do 2 apply elem_of_union_l.
-    apply elem_of_singleton_2.
     rewrite HIn.
-    reflexivity.
+    set_solver +.
     apply finz_succN_in_seq; simpl; lia.
-    rewrite HIn.
-    rewrite to_pid_aligned_eq.
-    assumption.
+    rewrite HIn. done.
     apply finz_succN_in_seq; simpl; lia.
     iFrame.
     iModIntro.
@@ -1755,24 +1661,23 @@ Section proof.
     iEval (rewrite finz_plus_one_simpl) in "PCs".
     rewrite Z_of_nat_simpl.
     iEval (simpl) in "PCs".
-    iApply ((@str _ _ _ _ _ _ _ four two 1%Qp prx1 (tpa p_tx1) ({[pshare]} ∪ {[p_pg1; tpa p_tx1; tpa prx1]}) (p_pg1 ^+ 9%nat)%f addr R3 R5) with "[p_10 PCs acc mem RX1page tx R3s R5s]").
+    iApply ((@str _ _ _ _ _ _ _ four two 1%Qp prx1 ptx1 ({[pshare]} ∪ {[pprog1; ptx1; prx1]}) (pprog1 ^+ 9%nat)%f addr R3 R5) with "[p_10 PCs acc mem RX1page tx R3s R5s]").
     apply decode_encode_instruction.
-    apply union_subseteq.
-    split; rewrite singleton_subseteq_l.
-    apply elem_of_union_l.
-    apply elem_of_singleton_2.
-    reflexivity.    
-    apply elem_of_union_r.
-    do 2 apply elem_of_union_l.
-    apply elem_of_singleton_2.
-    rewrite (finz_succN_pid' p_pg1 9).
-    reflexivity.
-    lia.    
-    rewrite HIn.
+    rewrite -Heq_pshare.
     rewrite to_pid_aligned_eq.
-    assumption.
+    rewrite (finz_succN_pid' pprog1 9);[|lia].
+    set_solver +.
+    rewrite HIn. done.
     apply finz_succN_in_seq; simpl; lia.
-    assumption.    
+    rewrite -Heq_pshare.
+    rewrite to_pid_aligned_eq.
+    {
+      intros Heq.
+      feed pose proof (NoDup_lookup _ 3 8 prx1 Hps_nd).
+      rewrite Heq. done.
+      rewrite Heq. done.
+      lia.
+    }
     iFrame.
     iModIntro.
     iIntros "(PCs & _ & R5s & mem & R3s & acc & tx & RX1page) _".
@@ -1780,18 +1685,13 @@ Section proof.
     iEval (rewrite finz_plus_one_simpl) in "PCs".
     rewrite Z_of_nat_simpl.
     iEval (simpl) in "PCs".
-    iApply ((mov_word (w3 := encode_hvc_ret_code Succ) (p_tx := p_tx1) (w1 := mov_word_I R0 msg_poll_I) (q := 1%Qp) (s := {[pshare]} ∪ {[p_pg1; tpa p_tx1; tpa prx1]}) (p_pg1 ^+ 10%nat)%f msg_poll_I R0) with "[p_11 PCs acc tx R0s]").
+    iApply ((mov_word (w3 := encode_hvc_ret_code Succ) (p_tx := ptx1) (w1 := mov_word_I R0 msg_poll_I) (q := 1%Qp) (s := {[pshare]} ∪ {[pprog1; ptx1; prx1]}) (pprog1 ^+ 10%nat)%f msg_poll_I R0) with "[p_11 PCs acc tx R0s]").
     by rewrite decode_encode_instruction.
-    apply elem_of_union_r.
-    do 2 apply elem_of_union_l.
-    apply elem_of_singleton_2.    
     rewrite HIn.
-    reflexivity.
+    set_solver +.
     apply finz_succN_in_seq; simpl; lia.
-    rewrite HIn.
-    assumption.
+    rewrite HIn. done.
     apply finz_succN_in_seq; simpl; lia.
-    rewrite to_pid_aligned_eq.
     iFrame.
     iModIntro.
     iIntros "(PCs & _ & acc & tx & R0s) _".
@@ -1799,15 +1699,11 @@ Section proof.
     iEval (rewrite finz_plus_one_simpl) in "PCs".
     rewrite Z_of_nat_simpl.
     iEval (simpl) in "PCs".
-    iApply ((msg_poll_full (r0 := msg_poll_I) (r1 := wh) (r2 := encode_vmid V0) (wi := hvc_I) (l := l) (i := V1) (j := V0) (p_tx := p_tx1) (q := 1%Qp) (s := {[pshare]} ∪ {[p_pg1; tpa p_tx1; tpa prx1]}) (p_pg1 ^+ 11%nat)%f) with "[p_12 PCs acc tx R0s R1s R2s RX1st]").
-    apply elem_of_union_r.
-    do 2 apply elem_of_union_l.
-    apply elem_of_singleton_2.    
+    iApply ((msg_poll_full (r0 := msg_poll_I) (r1 := wh) (r2 := encode_vmid V0) (wi := hvc_I) (l := l) (i := V1) (j := V0) (p_tx := ptx1) (q := 1%Qp) (s := {[pshare]} ∪ {[pprog1; ptx1; prx1]}) (pprog1 ^+ 11%nat)%f) with "[p_12 PCs acc tx R0s R1s R2s RX1st]").
     rewrite HIn.
-    reflexivity.
+    set_solver +.
     apply finz_succN_in_seq; simpl; lia.
-    rewrite HIn.
-    assumption.
+    rewrite HIn. done.
     apply finz_succN_in_seq; simpl; lia.
     by rewrite decode_encode_instruction.
     by rewrite decode_encode_hvc_func.
@@ -1819,19 +1715,13 @@ Section proof.
     iEval (rewrite finz_plus_one_simpl) in "PCs".
     rewrite Z_of_nat_simpl.
     iEval (simpl) in "PCs".
-    iApply ((@mov_word _ _ _ _ _ _ _ _ _ ({[pshare]} ∪ {[p_pg1; tpa p_tx1; tpa prx1]}) (tpa p_tx1) (p_pg1 ^+ 12%nat)%f yield_I R0) with "[p_13 PCs acc tx R0s]").
+    iApply ((@mov_word _ _ _ _ _ _ _ _ _ ({[pshare]} ∪ {[pprog1; ptx1; prx1]}) ptx1 (pprog1 ^+ 12%nat)%f yield_I R0) with "[p_13 PCs acc tx R0s]").
     apply decode_encode_instruction.
-    apply elem_of_union_r.
-    do 2 apply elem_of_union_l.
-    apply elem_of_singleton_2.
     rewrite HIn.
-    reflexivity.
+    set_solver +.
     apply finz_succN_in_seq; simpl; lia.
-    rewrite HIn.
-    rewrite to_pid_aligned_eq.
-    assumption.
+    rewrite HIn. done.
     apply finz_succN_in_seq; simpl; lia.
-    rewrite to_pid_aligned_eq.
     iFrame.
     iModIntro.
     iIntros "(PCs & _ & acc & tx & R0s) _".
@@ -1839,16 +1729,11 @@ Section proof.
     iEval (rewrite finz_plus_one_simpl) in "PCs".
     rewrite Z_of_nat_simpl.
     iEval (simpl) in "PCs".
-    iApply ((yield (s := {[pshare]} ∪ {[p_pg1; tpa p_tx1; tpa prx1]}) (p_tx := tpa p_tx1) (p_pg1 ^+ 13%nat)%f True False%I) with "[PCs p_14 acc tx R0s R0z R1z prop0 prop1 mem whtrans RX1page RX1st RX1mem]").
-    apply elem_of_union_r.
-    do 2 apply elem_of_union_l.
-    apply elem_of_singleton_2.
+    iApply ((yield (s := {[pshare]} ∪ {[pprog1; ptx1; prx1]}) (p_tx := ptx1) (pprog1 ^+ 13%nat)%f True False%I) with "[PCs p_14 acc tx R0s R0z R1z prop0 prop1 mem whtrans RX1page RX1st RX1mem]").
     rewrite HIn.
-    reflexivity.
+    set_solver +.
     apply finz_succN_in_seq; simpl; lia.
-    rewrite HIn.
-    rewrite to_pid_aligned_eq.
-    assumption.
+    rewrite HIn. done.
     apply finz_succN_in_seq; simpl; lia.
     done.
     apply decode_encode_instruction.
@@ -1856,8 +1741,8 @@ Section proof.
     {
       iSplitL "PCs p_14 acc tx R0s R0z R1z".
       iFrame.
-      iFrame "prop0".
-      iFrame "prop1".
+      iSplitL "prop0". iExact "prop0".
+      iSplitL "prop1". iExact "prop1".
       iSplit; last done.
       iNext.
       iIntros "((H1 & H2 & H3 & H4 & H5 & H6 & H7) & _ & H8)".
@@ -1879,5 +1764,12 @@ Section proof.
     iMod "P".
     by iExFalso.
   Qed.
-  
+
+  Definition mtms_interp_access2 := interp_access (V2 : leibnizO VMID)
+                                                  mtms_slice_trans mtms_slice_rxs
+                                      ptx2 prx2 {[pprog2; ptx2; prx2]} ∅.
+
+
+  Lemma mtms_ftlr2 : mtms_interp_access2 ⊢ interp_execute V2.
+  Proof. iApply ftlr. Qed.
 End proof.
